<?xml version="1.0" encoding="utf-8"?>
<rdf:RDF xml:base="http://iirds.tekom.de/iirds#" xml:lang="en" xmlns:iirds="http://iirds.tekom.de/iirds#"  xmlns:rdf="http://www.w3.org/1999/02/22-rdf-syntax-ns#" xmlns:rdfs="http://www.w3.org/2000/01/rdf-schema#" xmlns:schema="http://schema.org/">

<!--
© 2023 Gesellschaft für Technische Kommunikation – tekom Deutschland e.V. All rights reserved.
This work is licensed under a Creative Commons Attribution-NoDerivatives 4.0 International License (https://creativecommons.org/licenses/by-nd/4.0/).
-->
	<rdfs:Class rdf:about="http://iirds.tekom.de/iirds#Action">
		<rdfs:label xml:lang="de">Handlung</rdfs:label>
		<rdfs:label xml:lang="en">action</rdfs:label>
		<rdfs:subClassOf rdf:resource="http://iirds.tekom.de/iirds#FunctionalMetadata"/>
		<iirds:description xml:lang="en">Use the relates-to-action property to create a reference from an information unit to an action.</iirds:description>
		<rdfs:comment xml:lang="en">atomic manipulation of an object by a participant</rdfs:comment>
	</rdfs:Class>
	<rdfs:Class rdf:about="http://iirds.tekom.de/iirds#AdministrativeMetadata">
		<rdfs:label xml:lang="de">Verwaltungsmetadaten</rdfs:label>
		<rdfs:label xml:lang="en">administrative metadata</rdfs:label>
		<rdfs:subClassOf rdf:resource="http://iirds.tekom.de/iirds#iirdsDomainEntity"/>
		<iirds:description xml:lang="en">Not intended to be used directly. Use the subclasses instead.</iirds:description>
		<rdfs:comment xml:lang="en">information that allows the management of iiRDS resources</rdfs:comment>
	</rdfs:Class>
	<rdfs:Class rdf:about="http://iirds.tekom.de/iirds#AfterUse">
		<rdfs:label xml:lang="de">Nutzungsende</rdfs:label>
		<rdfs:label xml:lang="en">after use</rdfs:label>
		<rdfs:subClassOf rdf:resource="http://iirds.tekom.de/iirds#ProductLifeCyclePhase"/>
		<iirds:description xml:lang="en">Not intended to be used directly. Use the subclasses instead. For lifecycle phases not covered by the iiRDS standard subclasses, define custom subclasses.</iirds:description>
		<rdfs:comment xml:lang="en">product life cycle phase that follows the active use of the product</rdfs:comment>
		<iirds:description xml:lang="en">IRI: required</iirds:description>
	</rdfs:Class>
	<rdfs:Class rdf:about="http://iirds.tekom.de/iirds#Collection">
		<rdfs:label xml:lang="de">Zusammenstellung</rdfs:label>
		<rdfs:label xml:lang="en">collection</rdfs:label>
		<rdfs:subClassOf rdf:resource="http://iirds.tekom.de/iirds#InformationSubject"/>
		<iirds:description xml:lang="en">Not intented to be used directly. Use the subclasses instead. For collection subjects not covered by the iiRDS standard subclasses, define custom subclasses.</iirds:description>
		<rdfs:comment xml:lang="en">information subject that covers specific content in lists or overviews</rdfs:comment>
		<iirds:description xml:lang="en">IRI: required</iirds:description>
	</rdfs:Class>
	<rdfs:Class rdf:about="http://iirds.tekom.de/iirds#Component">
		<rdfs:label xml:lang="de">Komponente</rdfs:label>
		<rdfs:label xml:lang="en">component</rdfs:label>
		<rdfs:subClassOf rdf:resource="http://iirds.tekom.de/iirds#ProductMetadata"/>
		<iirds:description xml:lang="en">Components may have relations to other components so that iiRDS Generators can build up a simple component hierarchy with iiRDS structures. The iirds#Component may also be used as a docking point for external component definitions.</iirds:description>
		<rdfs:comment xml:lang="en">part used as a constituent in an assembled product, system or plant</rdfs:comment>
		<iirds:description xml:lang="en">IRI: required</iirds:description>
	</rdfs:Class>
	<rdfs:Class rdf:about="http://iirds.tekom.de/iirds#Concept">
		<rdfs:label xml:lang="de">Beschreibung</rdfs:label>
		<rdfs:label xml:lang="en">concept</rdfs:label>
		<rdfs:subClassOf rdf:resource="http://iirds.tekom.de/iirds#TopicType"/>
		<iirds:description xml:lang="en">Conceptual information helps users to map their existing knowledge to tasks and other essential information about a product or system.
		</iirds:description>
		<rdfs:comment xml:lang="en">topic type that provides background information which helps users understand the structure or essential principles of a product, interface, or task</rdfs:comment>
		<iirds:description xml:lang="en">IRI: required</iirds:description>
	</rdfs:Class>
	<rdfs:Class rdf:about="http://iirds.tekom.de/iirds#Conformity">
		<rdfs:label xml:lang="de">Konformität</rdfs:label>
		<rdfs:label xml:lang="en">conformity</rdfs:label>
		<rdfs:subClassOf rdf:resource="http://iirds.tekom.de/iirds#InformationSubject"/>
		<iirds:description xml:lang="en">Not intended to be used directly. Use the subclasses instead. For information subjects not covered by the iiRDS standard subclasses, define custom subclasses.</iirds:description>
		<rdfs:comment xml:lang="en">information subject that covers applicable standards or the fulfilment of a product requirement</rdfs:comment>
		<iirds:description xml:lang="en">IRI: required</iirds:description>
	</rdfs:Class>
	<rdfs:Class rdf:about="http://iirds.tekom.de/iirds#DesignAndRealization">
		<rdfs:label xml:lang="de">Produktentstehung</rdfs:label>
		<rdfs:label xml:lang="en">design and realization</rdfs:label>
		<rdfs:subClassOf rdf:resource="http://iirds.tekom.de/iirds#ProductLifeCyclePhase"/>
		<iirds:description xml:lang="en">Not intended to be used directly. Use the subclasses instead. For lifecycle phases not covered by the iiRDS standard subclasses, define custom subclasses.</iirds:description>
		<rdfs:comment xml:lang="en">product life cycle phase from environment analysis and ideation through production</rdfs:comment>
		<iirds:description xml:lang="en">IRI: required</iirds:description>
	</rdfs:Class>
	<rdfs:Class rdf:about="http://iirds.tekom.de/iirds#DirectoryNode">
		<rdfs:label xml:lang="de">Verzeichnisknoten</rdfs:label>
		<rdfs:label xml:lang="en">directory node</rdfs:label>
		<rdfs:subClassOf rdf:resource="http://iirds.tekom.de/iirds#iirdsDomainEntity"/>
		<iirds:description xml:lang="en">A directory is a tree-like, ordered collection of information units. Directory nodes are the entries in the directory. Directories help the user to navigate through the information units. A table of contents is a typical example of a directory. </iirds:description>
		<iirds:description xml:lang="de">Ein Verzeichnis ist eine baumartig organisierte und geordnete Zusammenstellung von Informationseinheiten. Verzeichnisknoten sind die Einträge in dem Baum. Verzeichnisse dienen dem Benutzer als Navigationshilfe über die Informationseinheiten. Ein Inhaltsverzeichnis eines Dokuments ist ein typisches Beispiel eines Verzeichnisses.</iirds:description>
		<rdfs:comment xml:lang="en">node in a tree-like, ordered collection</rdfs:comment>
		<iirds:description xml:lang="en">IRI: optional</iirds:description>
	</rdfs:Class>
	<rdfs:Class rdf:about="http://iirds.tekom.de/iirds#DirectoryNodeType">
		<rdfs:label xml:lang="de">Verzeichnistyp</rdfs:label>
		<rdfs:label xml:lang="en">directory node type</rdfs:label>
		<rdfs:subClassOf rdf:resource="http://iirds.tekom.de/iirds#InformationType"/>
		<iirds:description xml:lang="en">A directory represented by a directory root node and its sub nodes has a type such as 'table of contens' or 'list of figures'.</iirds:description>
		<iirds:description xml:lang="de">Ein Verzeichnis, das durch einen Wurzelknoten und seine untergeordneten Knoten aufgespannt wird, hat einen Typ wie 'Inhaltsverzeichnis' oder 'Abbildungsverzeichnis'.</iirds:description>
		<rdfs:comment xml:lang="en">type of information arranged in a hierarchically ordered list of elements built by a root node and its subordinate nodes</rdfs:comment>
		<iirds:description xml:lang="en">IRI: required</iirds:description>
	</rdfs:Class>
	<rdfs:Class rdf:about="http://iirds.tekom.de/iirds#Document">
		<rdfs:label xml:lang="de">Dokument</rdfs:label>
		<rdfs:label xml:lang="en">document</rdfs:label>
		<rdfs:subClassOf rdf:resource="http://iirds.tekom.de/iirds#InformationUnit"/>
		<iirds:description xml:lang="en">A document consists of one or more files. It can consist of topics. The resource is either a blank node (when there is no file representing the document) or a file in the iiRDS package.</iirds:description>
		<rdfs:comment xml:lang="en">information unit that consists of an ordered set of information intended by the sender to be regarded as an entity</rdfs:comment>
		<iirds:description xml:lang="en">IRI: required</iirds:description>
	</rdfs:Class>
	<rdfs:Class rdf:about="http://iirds.tekom.de/iirds#DocumentationMetadata">
		<rdfs:label xml:lang="de">Metadaten der Dokumentation</rdfs:label>
		<rdfs:label xml:lang="en">documentation metadata</rdfs:label>
		<rdfs:subClassOf rdf:resource="http://iirds.tekom.de/iirds#iirdsDomainEntity"/>
		<iirds:description xml:lang="en">Not intended to be used directly. Use the subclasses instead.</iirds:description>
		<rdfs:comment xml:lang="en">information that describes the context to which iiRDS resources apply</rdfs:comment>
	</rdfs:Class>
	<rdfs:Class rdf:about="http://iirds.tekom.de/iirds#DocumentType">
		<rdfs:label xml:lang="de">Dokumentart</rdfs:label>
		<rdfs:label xml:lang="en">document type</rdfs:label>
		<rdfs:subClassOf rdf:resource="http://iirds.tekom.de/iirds#InformationType"/>
		<iirds:description xml:lang="en">Document types define the intended purpose of a document.</iirds:description>
		<rdfs:comment xml:lang="en">type of information arranged in a document defined with respect to its specified purpose, function, and form of presentation</rdfs:comment>
		<iirds:description xml:lang="en">IRI: required</iirds:description>
	</rdfs:Class>
	<rdfs:Class rdf:about="http://iirds.tekom.de/iirds#DownTime">
		<rdfs:label xml:lang="de">Stillstandzeit</rdfs:label>
		<rdfs:label xml:lang="en">down time</rdfs:label>
		<rdfs:subClassOf rdf:resource="http://iirds.tekom.de/iirds#PlanningTime"/>
		<iirds:description xml:lang="en"/>
		<rdfs:comment xml:lang="en">period of time during which an item is not in condition to perform its intended function</rdfs:comment>
		<iirds:description xml:lang="en">IRI: optional</iirds:description>
	</rdfs:Class>
	<rdfs:Class rdf:about="http://iirds.tekom.de/iirds#Event">
		<rdfs:label xml:lang="de">Ereignis</rdfs:label>
		<rdfs:label xml:lang="en">event</rdfs:label>
		<rdfs:subClassOf rdf:resource="http://iirds.tekom.de/iirds#FunctionalMetadata"/>
		<iirds:description xml:lang="en">Examples are errors, malfunctions, and warnings.
Use the relates-to-event property to create a reference from an information unit to an event.</iirds:description>
		<rdfs:comment xml:lang="en">something noticeable that takes place at a given location and point in time</rdfs:comment>
		<iirds:description xml:lang="en">IRI: required</iirds:description>
	</rdfs:Class>
	<rdfs:Class rdf:about="http://iirds.tekom.de/iirds#ContentLifeCycleStatus">
		<rdfs:label xml:lang="de">Lebenszyklus-Status einer Informationseinheit</rdfs:label>
		<rdfs:label xml:lang="en">information unit lifecycle status</rdfs:label>
		<rdfs:subClassOf rdf:resource="http://iirds.tekom.de/iirds#AdministrativeMetadata"/>
		<iirds:description xml:lang="en">The status value is referenced using has-content-lifecycle-status-value. </iirds:description>
		<rdfs:comment xml:lang="en">stage of an information unit in the information development process</rdfs:comment>
		<iirds:description xml:lang="en">IRI: optional</iirds:description>
	</rdfs:Class>
	<rdfs:Class rdf:about="http://iirds.tekom.de/iirds#ContentLifeCycleStatusValue">
		<rdfs:label xml:lang="de">Wert des Lebenszyklus-Status einer Informationseinheit</rdfs:label>
		<rdfs:label xml:lang="en">value of the information unit lifecycle status</rdfs:label>
		<rdfs:subClassOf rdf:resource="http://iirds.tekom.de/iirds#AdministrativeMetadata"/>
		<iirds:description xml:lang="en">The value refers to the content status, for example whether it is approved or withdrawn.</iirds:description>
		<rdfs:comment xml:lang="en">categorical denomination of the information unit life cycle stage</rdfs:comment>
		<iirds:description xml:lang="en">IRI: required</iirds:description>
	</rdfs:Class>
	<rdfs:Class rdf:about="http://iirds.tekom.de/iirds#Identity">
		<rdfs:label xml:lang="de">Identität</rdfs:label>
		<rdfs:label xml:lang="en">identity</rdfs:label>
		<rdfs:subClassOf rdf:resource="http://iirds.tekom.de/iirds#AdministrativeMetadata"/>
		<iirds:description xml:lang="en">Complex identifiers may be assigned to information objects, information units, product variants, and components. Typically, identities are used to provide IDs from other systems. Examples: serial numbers for components and module IDs from content management systems for topics.</iirds:description>
		<rdfs:comment xml:lang="en">complex identifier of a resource in an external system</rdfs:comment>
		<iirds:description xml:lang="en">IRI: optional</iirds:description>
	</rdfs:Class>
	<rdfs:Class rdf:about="http://iirds.tekom.de/iirds#IdentityDomain">
		<rdfs:label xml:lang="de">Identitäts-Domäne</rdfs:label>
		<rdfs:label xml:lang="en">identity domain</rdfs:label>
		<rdfs:subClassOf rdf:resource="http://iirds.tekom.de/iirds#AdministrativeMetadata"/>
		<iirds:description xml:lang="en">An identity domain relates to a party, meaning a company or organization. The party is the owner or custodian of the domain.</iirds:description>
		<rdfs:comment xml:lang="en">organizational origin of an identifier that is assigned to an iiRDS identity</rdfs:comment>
		<iirds:description xml:lang="en">IRI: required</iirds:description>
	</rdfs:Class>
	<rdfs:Class rdf:about="http://iirds.tekom.de/iirds#IdentityType">
		<rdfs:label xml:lang="de">Identitäts-Typ</rdfs:label>
		<rdfs:label xml:lang="en">identity type</rdfs:label>
		<rdfs:subClassOf rdf:resource="http://iirds.tekom.de/iirds#AdministrativeMetadata"/>
		<iirds:description xml:lang="en">The type of identity contained by the domain.</iirds:description>
		<rdfs:comment xml:lang="en">distinguished set of identifiers that are assigned to an iiRDS identity</rdfs:comment>
		<iirds:description xml:lang="en">IRI: required</iirds:description>
	</rdfs:Class>
	<rdfs:Class rdf:about="http://iirds.tekom.de/iirds#ExternalClassification">
		<rdfs:label xml:lang="de">Externe Klassifikation</rdfs:label>
		<rdfs:label xml:lang="en">external classification</rdfs:label>
		<rdfs:subClassOf rdf:resource="http://iirds.tekom.de/iirds#AdministrativeMetadata"/>
		<iirds:description xml:lang="en">External classifications may be assigned to information objects, information units, product variants, product features and components. Typically, external classifications are used to include metadata from other standards. Examples: ECLASS and CDD (IEC 61360) for product classfication and DCC (IEC 61355) or VDI 2770 for document classification.</iirds:description>
		<rdfs:comment xml:lang="en">External classification of an iiRDS domain entity. Each classification must be related to the classification domain within which it is unambiguous.</rdfs:comment>
		<iirds:description xml:lang="en">IRI: optional</iirds:description>
	</rdfs:Class>
	<rdfs:Class rdf:about="http://iirds.tekom.de/iirds#ClassificationDomain">
		<rdfs:label xml:lang="de">Externe Klassifikationsdomäne</rdfs:label>
		<rdfs:label xml:lang="en">external classification domain</rdfs:label>
		<rdfs:subClassOf rdf:resource="http://iirds.tekom.de/iirds#AdministrativeMetadata"/>
		<iirds:description xml:lang="en">A classification domain relates to a party, meaning a company or organization. The party is the owner or custodian of the domain.</iirds:description>
		<rdfs:comment xml:lang="en">domain of an external classification that is assigned to an iiRDS entity</rdfs:comment>
		<iirds:description xml:lang="en">IRI: required</iirds:description>
	</rdfs:Class>
	<rdfs:Class rdf:about="http://iirds.tekom.de/iirds#ClassificationType">
		<rdfs:label xml:lang="de">Klassifikationstyp</rdfs:label>
		<rdfs:label xml:lang="en">classification type</rdfs:label>
		<rdfs:subClassOf rdf:resource="http://iirds.tekom.de/iirds#AdministrativeMetadata"/>
		<iirds:description xml:lang="en">The type of classification contained by the domain.</iirds:description>
		<rdfs:comment xml:lang="en">type of an classification that is assigned to an iiRDS domain entity</rdfs:comment>
		<iirds:description xml:lang="en">IRI: required</iirds:description>
	</rdfs:Class>
	<rdfs:Class rdf:about="http://iirds.tekom.de/iirds#Form">
		<rdfs:label xml:lang="de">Formular</rdfs:label>
		<rdfs:label xml:lang="en">form</rdfs:label>
		<rdfs:subClassOf rdf:resource="http://iirds.tekom.de/iirds#TopicType"/>
		<iirds:description xml:lang="en">Examples of forms are service reports, field reports, and user feedback.</iirds:description>
		<rdfs:comment xml:lang="en">topic type that provides information in pre-defined fields</rdfs:comment>
		<iirds:description xml:lang="en">IRI: required</iirds:description>
	</rdfs:Class>
	<rdfs:Class rdf:about="http://iirds.tekom.de/iirds#Formality">
		<rdfs:label xml:lang="de">Formalität</rdfs:label>
		<rdfs:label xml:lang="en">formality</rdfs:label>
		<rdfs:subClassOf rdf:resource="http://iirds.tekom.de/iirds#InformationSubject"/>
		<iirds:description xml:lang="en">Examples of formality subjects are license terms and warranty conditions.</iirds:description>
		<rdfs:comment xml:lang="en">information subject that covers contractually relevant elements</rdfs:comment>
		<iirds:description xml:lang="en">IRI: required</iirds:description>
	</rdfs:Class>
	<rdfs:Class rdf:about="http://iirds.tekom.de/iirds#Fragment">
		<rdfs:label xml:lang="de">Fragment</rdfs:label>
		<rdfs:label xml:lang="en">fragment</rdfs:label>
		<rdfs:subClassOf rdf:resource="http://iirds.tekom.de/iirds#InformationUnit"/>
		<iirds:description xml:lang="en">Sections, tables, lists, paragraphs, and hazard statements are examples of fragments. Fragments assign metadata to parts of topic or document files in an iiRDS package. The parts are identified by a fragment selector.</iirds:description>
		<rdfs:comment xml:lang="en">information unit that requires additional context</rdfs:comment>
		<iirds:description xml:lang="en">IRI: required</iirds:description>
	</rdfs:Class>
	<rdfs:Class rdf:about="http://iirds.tekom.de/iirds#FragmentSelector">
		<rdfs:label xml:lang="de">Fragmentselektor</rdfs:label>
		<rdfs:label xml:lang="en">fragment selector</rdfs:label>
		<rdfs:subClassOf rdf:resource="http://iirds.tekom.de/iirds#Selector"/>
		<rdfs:comment xml:lang="en">selector that defines a part of content by a single identifier</rdfs:comment>
		<iirds:description xml:lang="en">IRI: optional</iirds:description>
	</rdfs:Class>
	<rdfs:Class rdf:about="http://iirds.tekom.de/iirds#Functionality">
		<rdfs:label xml:lang="de">Funktionalität</rdfs:label>
		<rdfs:label xml:lang="en">functionality</rdfs:label>
		<rdfs:subClassOf rdf:resource="http://iirds.tekom.de/iirds#InformationSubject"/>
		<iirds:description xml:lang="en"/>
		<rdfs:comment xml:lang="en">information subject that covers specific capabilities of the product</rdfs:comment>
		<iirds:description xml:lang="en">IRI: required</iirds:description>
	</rdfs:Class>
	<rdfs:Class rdf:about="http://iirds.tekom.de/iirds#FunctionalMetadata">
		<rdfs:label xml:lang="de">Funktionale Metadaten</rdfs:label>
		<rdfs:label xml:lang="en">functional metadata</rdfs:label>
		<rdfs:subClassOf rdf:resource="http://iirds.tekom.de/iirds#DocumentationMetadata"/>
		<iirds:description xml:lang="en">Not intended to be used directly. Use the subclasses instead.</iirds:description>
		<rdfs:comment xml:lang="en">information used to implement advanced content delivery scenarios and content assemblies for specific purposes</rdfs:comment>
	</rdfs:Class>
	<rdfs:Class rdf:about="http://iirds.tekom.de/iirds#iirdsDomainEntity">
		<rdfs:label xml:lang="de">iirdsDomainEntity</rdfs:label>
		<rdfs:label xml:lang="en">iirdsDomainEntity</rdfs:label>
		<iirds:description xml:lang="en">Not intended to be used directly. Use the subclasses instead.</iirds:description>
		<rdfs:comment xml:lang="en">any resource within the iiRDS domain</rdfs:comment>
	</rdfs:Class>
	<rdfs:Class rdf:about="http://iirds.tekom.de/iirds#InformationObject">
		<rdfs:label xml:lang="de">Informationsobjekt</rdfs:label>
		<rdfs:label xml:lang="en">information object</rdfs:label>
		<rdfs:subClassOf rdf:resource="http://iirds.tekom.de/iirds#iirdsDomainEntity"/>
		<iirds:description xml:lang="en">Only used if a version/language-independent equivalent to an information unit is required. The versioned information unit references the information object.</iirds:description>
		<rdfs:comment xml:lang="en">version- and language-independent abstraction of an information unit</rdfs:comment>
		<iirds:description xml:lang="en">IRI: required</iirds:description>
	</rdfs:Class>
	<rdfs:Class rdf:about="http://iirds.tekom.de/iirds#InformationSubject">
		<rdfs:label xml:lang="de">Informationsthema</rdfs:label>
		<rdfs:label xml:lang="en">information subject</rdfs:label>
		<rdfs:subClassOf rdf:resource="http://iirds.tekom.de/iirds#InformationType"/>
		<iirds:description xml:lang="en">Not intented to be used directly. Use the subclasses instead.</iirds:description>
		<rdfs:comment xml:lang="en">thematical characteristic of content</rdfs:comment>
		<iirds:description xml:lang="en">IRI: required</iirds:description>
	</rdfs:Class>
	<rdfs:Class rdf:about="http://iirds.tekom.de/iirds#InformationType">
		<rdfs:label xml:lang="de">Informationsart</rdfs:label>
		<rdfs:label xml:lang="en">information type</rdfs:label>
		<rdfs:subClassOf rdf:resource="http://iirds.tekom.de/iirds#iirdsDomainEntity"/>
		<iirds:description xml:lang="en">Not intented to be used directly.</iirds:description>
		<rdfs:comment xml:lang="en">characteristic of content</rdfs:comment>
		<iirds:description xml:lang="en">IRI: required</iirds:description>
	</rdfs:Class>
	<rdfs:Class rdf:about="http://iirds.tekom.de/iirds#InformationUnit">
		<rdfs:label xml:lang="de">Informationseinheit</rdfs:label>
		<rdfs:label xml:lang="en">information unit</rdfs:label>
		<rdfs:subClassOf rdf:resource="http://iirds.tekom.de/iirds#iirdsDomainEntity"/>
		<iirds:description xml:lang="en">Not intended to be used directly. Use the subclasses Package, Document, Topic, and Fragment instead.</iirds:description>
		<rdfs:comment xml:lang="en">piece of digitally encoded information</rdfs:comment>
		<iirds:description xml:lang="en">IRI: required</iirds:description>
	</rdfs:Class>
	<rdfs:Class rdf:about="http://iirds.tekom.de/iirds#Learning">
		<rdfs:label xml:lang="de">Lernen</rdfs:label>
		<rdfs:label xml:lang="en">learning</rdfs:label>
		<rdfs:subClassOf rdf:resource="http://iirds.tekom.de/iirds#TopicType"/>
		<iirds:description xml:lang="en">Learning content may comprise learning plans, learning objectives, learning content details, summaries, and assessments.</iirds:description>
		<rdfs:comment xml:lang="en">topic type that provides learning content</rdfs:comment>
		<iirds:description xml:lang="en">IRI: required</iirds:description>
	</rdfs:Class>
	<rdfs:Class rdf:about="http://iirds.tekom.de/iirds#MaintenanceInterval">
		<rdfs:label xml:lang="de">Wartungsintervall</rdfs:label>
		<rdfs:label xml:lang="en">maintenance interval</rdfs:label>
		<rdfs:subClassOf rdf:resource="http://iirds.tekom.de/iirds#PlanningTime"/>
		<iirds:description xml:lang="en">Instances have a maintenance frequency and an optional maintenance duration.</iirds:description>
		<rdfs:comment xml:lang="en">period of time between scheduled maintenance operations</rdfs:comment>
		<iirds:description xml:lang="en">IRI: optional</iirds:description>
	</rdfs:Class>
	<rdfs:Class rdf:about="http://iirds.tekom.de/iirds#nil">
		<rdfs:label xml:lang="de">Ende einer Verzeichnisstruktur</rdfs:label>
		<rdfs:label xml:lang="en">end of Directory node</rdfs:label>
		<rdfs:subClassOf rdf:resource="http://iirds.tekom.de/iirds#DirectoryNode"/>
		<iirds:description xml:lang="en"/>
		<rdfs:comment xml:lang="en">closing element in a chain of directory nodes</rdfs:comment>
	</rdfs:Class>
	<rdfs:Class rdf:about="http://iirds.tekom.de/iirds#Package">
		<rdfs:label xml:lang="de">Paket</rdfs:label>
		<rdfs:label xml:lang="en">package</rdfs:label>
		<rdfs:subClassOf rdf:resource="http://iirds.tekom.de/iirds#InformationUnit"/>
		<iirds:description xml:lang="en">There is exactly one Package instance within an iiRDS package. It holds general metadata on the overall iiRDS package.</iirds:description>
		<rdfs:comment xml:lang="en">information unit that bundles other information units for exchange</rdfs:comment>
		<iirds:description xml:lang="en">IRI: required</iirds:description>
	</rdfs:Class>
	<rdfs:Class rdf:about="http://iirds.tekom.de/iirds#Party">
		<rdfs:label xml:lang="de">Akteur</rdfs:label>
		<rdfs:label xml:lang="en">party</rdfs:label>
		<rdfs:subClassOf rdf:resource="http://iirds.tekom.de/iirds#AdministrativeMetadata"/>
		<iirds:description xml:lang="en">Detailed information about a party may be specified in a vCard.</iirds:description>
		<rdfs:comment xml:lang="en">person, organization, or system</rdfs:comment>
		<iirds:description xml:lang="en">IRI: required</iirds:description>
	</rdfs:Class>
	<rdfs:Class rdf:about="http://iirds.tekom.de/iirds#PartyRole">
		<rdfs:label xml:lang="de">Akteursrolle</rdfs:label>
		<rdfs:label xml:lang="en">party role</rdfs:label>
		<rdfs:subClassOf rdf:resource="http://iirds.tekom.de/iirds#AdministrativeMetadata"/>
		<iirds:description xml:lang="en">Examples of party roles: manufacturer, author, inspector.</iirds:description>
		<rdfs:comment xml:lang="en">responsibility of a person or organization</rdfs:comment>
		<iirds:description xml:lang="en">IRI: required</iirds:description>
	</rdfs:Class>
	<rdfs:Class rdf:about="http://iirds.tekom.de/iirds#PlanningTime">
		<rdfs:label xml:lang="de">Planungszeit</rdfs:label>
		<rdfs:label xml:lang="en">planning time</rdfs:label>
		<rdfs:subClassOf rdf:resource="http://iirds.tekom.de/iirds#FunctionalMetadata"/>
		<iirds:description xml:lang="en">Not intended to be used directly.  Use the subclasses instead.</iirds:description>
		<rdfs:comment xml:lang="en">period of time required for or resulting from a specific task</rdfs:comment>
		<iirds:description xml:lang="en">IRI: optional</iirds:description>
	</rdfs:Class>
	<rdfs:Class rdf:about="http://iirds.tekom.de/iirds#Process">
		<rdfs:label xml:lang="de">Prozess</rdfs:label>
		<rdfs:label xml:lang="en">process</rdfs:label>
		<rdfs:subClassOf rdf:resource="http://iirds.tekom.de/iirds#InformationSubject"/>
		<iirds:description xml:lang="en"/>
		<rdfs:comment xml:lang="en">information subject that covers structured activities carried out to achieve a specific goal</rdfs:comment>
		<iirds:description xml:lang="en">IRI: required</iirds:description>
	</rdfs:Class>
	<rdfs:Class rdf:about="http://iirds.tekom.de/iirds#ProductFeature">
		<rdfs:label xml:lang="de">Produktmerkmal</rdfs:label>
		<rdfs:label xml:lang="en">product feature</rdfs:label>
		<rdfs:subClassOf rdf:resource="http://iirds.tekom.de/iirds#ProductMetadata"/>
		<iirds:description xml:lang="en">Not intended to be used directly. Use the subclasses instead.</iirds:description>
		<rdfs:comment xml:lang="en">product characteristics</rdfs:comment>
		<iirds:description xml:lang="en">IRI: required</iirds:description>
	</rdfs:Class>
	<rdfs:Class rdf:about="http://iirds.tekom.de/iirds#ProductProperty">
		<rdfs:label xml:lang="de">Produkteigenschaft</rdfs:label>
		<rdfs:label xml:lang="en">product property</rdfs:label>
		<rdfs:subClassOf rdf:resource="http://iirds.tekom.de/iirds#ProductFeature"/>
		<iirds:description xml:lang="en">Examples: dimensions, voltage, power, weight.</iirds:description>
		<rdfs:comment xml:lang="en">invariable characteristic of a product whose value is fixed once the product is defined</rdfs:comment>
		<iirds:description xml:lang="en">IRI: required</iirds:description>
	</rdfs:Class>
	<rdfs:Class rdf:about="http://iirds.tekom.de/iirds#ProductFunction">
		<rdfs:label xml:lang="de">Produktfunktion</rdfs:label>
		<rdfs:label xml:lang="en">product function</rdfs:label>
		<rdfs:subClassOf rdf:resource="http://iirds.tekom.de/iirds#ProductFeature"/>
		<iirds:description xml:lang="en">Examples: starting a phone call, ending a phone call, ringing.</iirds:description>
		<rdfs:comment xml:lang="en">capability of a product or a component which is specific or required for the intended product task</rdfs:comment>
		<iirds:description xml:lang="en">IRI: required</iirds:description>
	</rdfs:Class>
	<rdfs:Class rdf:about="http://iirds.tekom.de/iirds#ProductLifeCyclePhase">
		<rdfs:label xml:lang="de">Produktlebenszyklusphase</rdfs:label>
		<rdfs:label xml:lang="en">phase of product lifecycle</rdfs:label>
		<rdfs:subClassOf rdf:resource="http://iirds.tekom.de/iirds#ProductMetadata"/>
		<iirds:description xml:lang="en">Not intended to be used directly. Use the subclasses instead. </iirds:description>
		<rdfs:comment xml:lang="en">defined period in the evolution of a product from the conceptual idea to its ultimate disposal</rdfs:comment>
		<iirds:description xml:lang="en">IRI: required</iirds:description>
	</rdfs:Class>
	<rdfs:Class rdf:about="http://iirds.tekom.de/iirds#ProductMetadata">
		<rdfs:label xml:lang="de">Produktmetadaten</rdfs:label>
		<rdfs:label xml:lang="en">productMetadata</rdfs:label>
		<rdfs:subClassOf rdf:resource="http://iirds.tekom.de/iirds#DocumentationMetadata"/>
		<iirds:description xml:lang="en">Not intended to be used directly. Use the subclasses instead.</iirds:description>
		<rdfs:comment xml:lang="en">information about a product or component</rdfs:comment>
		<iirds:description xml:lang="en">IRI: required</iirds:description>
	</rdfs:Class>
	<rdfs:Class rdf:about="http://iirds.tekom.de/iirds#ProductVariant">
		<rdfs:label xml:lang="de">Produktvariante</rdfs:label>
		<rdfs:label xml:lang="en">product variant</rdfs:label>
		<rdfs:subClassOf rdf:resource="http://iirds.tekom.de/iirds#ProductMetadata"/>
		<iirds:description xml:lang="en">Examples: a specific model in a series or an individually manufactured good.</iirds:description>
		<rdfs:comment xml:lang="en">item or service offered on the market and designed to meet the needs or wishes of customers</rdfs:comment>
		<iirds:description xml:lang="en">IRI: required</iirds:description>
	</rdfs:Class>
	<rdfs:Class rdf:about="http://iirds.tekom.de/iirds#PuttingToUse">
		<rdfs:label xml:lang="de">In Nutzung nehmen</rdfs:label>
		<rdfs:label xml:lang="en">putting to use</rdfs:label>
		<rdfs:subClassOf rdf:resource="http://iirds.tekom.de/iirds#ProductLifeCyclePhase"/>
		<iirds:description xml:lang="en">Not intended to be used directly. Use the subclasses instead. For lifecycle phases not covered by the iiRDS standard subclasses, define custom subclasses.</iirds:description>
		<rdfs:comment xml:lang="en">product life cycle phase after production in which a product is set up for its intended use</rdfs:comment>
		<iirds:description xml:lang="en">IRI: required</iirds:description>
	</rdfs:Class>
	<rdfs:Class rdf:about="http://iirds.tekom.de/iirds#Qualification">
		<rdfs:label xml:lang="de">Qualifikation</rdfs:label>
		<rdfs:label xml:lang="en">qualification</rdfs:label>
		<rdfs:subClassOf rdf:resource="http://iirds.tekom.de/iirds#FunctionalMetadata"/>
		<iirds:description xml:lang="en">Not intended to be used directly. Use the subclasses instead. </iirds:description>
		<rdfs:comment xml:lang="en">proficiency, competence, or expertise exhibited by an individual</rdfs:comment>
		<iirds:description xml:lang="en">IRI: required</iirds:description>
	</rdfs:Class>
	<rdfs:Class rdf:about="http://iirds.tekom.de/iirds#RangeSelector">
		<rdfs:label xml:lang="de">Bereichsselektor</rdfs:label>
		<rdfs:label xml:lang="en">range selector</rdfs:label>
		<rdfs:subClassOf rdf:resource="http://iirds.tekom.de/iirds#Selector"/>
		<iirds:description xml:lang="en"/>
		<rdfs:comment xml:lang="en">selector that defines the start point and the end point of a part of content</rdfs:comment>
		<iirds:description xml:lang="en">IRI: optional</iirds:description>
	</rdfs:Class>
	<rdfs:Class rdf:about="http://iirds.tekom.de/iirds#Reference">
		<rdfs:label xml:lang="de">Referenz</rdfs:label>
		<rdfs:label xml:lang="en">reference</rdfs:label>
		<rdfs:subClassOf rdf:resource="http://iirds.tekom.de/iirds#TopicType"/>
		<iirds:description xml:lang="de">Examples are parameter lists, tables with technical data, UI control overviews, and parts lists.
		</iirds:description>
		<iirds:description xml:lang="en">IRI: required</iirds:description>
	</rdfs:Class>
	<rdfs:Class rdf:about="http://iirds.tekom.de/iirds#Rendition">
		<rdfs:label xml:lang="de">Inhaltsausprägung</rdfs:label>
		<rdfs:label xml:lang="en">rendition</rdfs:label>
		<rdfs:subClassOf rdf:resource="http://iirds.tekom.de/iirds#iirdsDomainEntity"/>
		<iirds:description xml:lang="en"/>
		<rdfs:comment xml:lang="en">content of an information unit in a specific format</rdfs:comment>
		<iirds:description xml:lang="en">IRI: optional</iirds:description>
	</rdfs:Class>
	<rdfs:Class rdf:about="http://iirds.tekom.de/iirds#Role">
		<rdfs:label xml:lang="de">Rolle</rdfs:label>
		<rdfs:label xml:lang="en">role</rdfs:label>
		<rdfs:subClassOf rdf:resource="http://iirds.tekom.de/iirds#Qualification"/>
		<iirds:description xml:lang="en">Describes a set of connected behaviors, privileges and obligations associated with users (humans, software processes or devices) of a system.</iirds:description>
		<iirds:description xml:lang="de">Menge von zusammenhängenden Verhaltensweisen, Berechtigungen und Verpflichtungen, die Nutzern (Menschen, Softwareprozesse oder Geräte) eines Systems zugeordnet sind.</iirds:description>
		<rdfs:comment xml:lang="en">set of connected behaviors, privileges, and obligations associated with a party</rdfs:comment>
		<iirds:description xml:lang="en">IRI: required</iirds:description>
	</rdfs:Class>
	<rdfs:Class rdf:about="http://iirds.tekom.de/iirds#Safety">
		<rdfs:label xml:lang="de">Sicherheit</rdfs:label>
		<rdfs:label xml:lang="en">safety</rdfs:label>
		<rdfs:subClassOf rdf:resource="http://iirds.tekom.de/iirds#InformationSubject"/>
		<iirds:description xml:lang="en">Not intended to be used directly. Use the subclasses instead.</iirds:description>
		<rdfs:comment xml:lang="en">information subject that covers content which helps to avoid risk</rdfs:comment>
		<iirds:description xml:lang="en">IRI: required</iirds:description>
	</rdfs:Class>
	<rdfs:Class rdf:about="http://iirds.tekom.de/iirds#WarningMessage">
		<rdfs:label xml:lang="de">Warnhinweis</rdfs:label>
		<rdfs:label xml:lang="en">warning message</rdfs:label>
		<rdfs:subClassOf rdf:resource="http://iirds.tekom.de/iirds#Safety"/>
		<iirds:description xml:lang="en">Warning messages usually consist of a hazard alert symbol, a signal word (such as "Danger", "Warning", "Caution", "Notice"),
a description of the potential hazard, and hints how to avoid the hazard.</iirds:description>
		<rdfs:comment xml:lang="en">safety-related information that warns about hazards and instructs on how to avoid them</rdfs:comment>
		<iirds:description xml:lang="en">IRI: required</iirds:description>
	</rdfs:Class>
	<rdfs:Class rdf:about="http://iirds.tekom.de/iirds#Selector">
		<rdfs:label xml:lang="de">Selektor</rdfs:label>
		<rdfs:label xml:lang="en">selector</rdfs:label>
		<rdfs:subClassOf rdf:resource="http://iirds.tekom.de/iirds#iirdsDomainEntity"/>
		<iirds:description xml:lang="en"/>
		<iirds:description xml:lang="de"/>
		<rdfs:comment xml:lang="en">pointer to the content of a rendition</rdfs:comment>
		<iirds:description xml:lang="en">IRI: optional</iirds:description>
	</rdfs:Class>
	<rdfs:Class rdf:about="http://iirds.tekom.de/iirds#SkillLevel">
		<rdfs:label xml:lang="de">Kenntnisstufe</rdfs:label>
		<rdfs:label xml:lang="en">skill level</rdfs:label>
		<rdfs:subClassOf rdf:resource="http://iirds.tekom.de/iirds#Qualification"/>
		<iirds:description xml:lang="en">Describe the levels of ability required to carry out a specific task described in the technical documentation.</iirds:description>
		<rdfs:comment xml:lang="en">degree of qualification of an individual</rdfs:comment>
		<iirds:description xml:lang="en">IRI: required</iirds:description>
	</rdfs:Class>
	<rdfs:Class rdf:about="http://iirds.tekom.de/iirds#Supply">
		<rdfs:label xml:lang="de">Hilfsmittel</rdfs:label>
		<rdfs:label xml:lang="en">supply</rdfs:label>
		<rdfs:subClassOf rdf:resource="http://iirds.tekom.de/iirds#FunctionalMetadata"/>
		<iirds:description xml:lang="en">Not intended to be used directly. Use the subclasses instead. </iirds:description>
		<rdfs:comment xml:lang="en">physical object used by an actor that performs work tasks described in technical documentation</rdfs:comment>
		<iirds:description xml:lang="en">IRI: required</iirds:description>
	</rdfs:Class>
	<rdfs:Class rdf:about="http://iirds.tekom.de/iirds#Task">
		<rdfs:label xml:lang="de">Aufgabe</rdfs:label>
		<rdfs:label xml:lang="en">task</rdfs:label>
		<rdfs:subClassOf rdf:resource="http://iirds.tekom.de/iirds#TopicType"/>
		<iirds:description xml:lang="en">Tasks provide instructions and may contain information on other aspects, such as requirements that must be fulfilled or safety instructions.
		</iirds:description>
		<rdfs:comment xml:lang="en">topic type that provides procedures and action steps to be followed or considered</rdfs:comment>
		<iirds:description xml:lang="en">IRI: required</iirds:description>
	</rdfs:Class>
	<rdfs:Class rdf:about="http://iirds.tekom.de/iirds#TechnicalData">
		<rdfs:label xml:lang="de">Technische Daten</rdfs:label>
		<rdfs:label xml:lang="en">technical data</rdfs:label>
		<rdfs:subClassOf rdf:resource="http://iirds.tekom.de/iirds#InformationSubject"/>
		<iirds:description xml:lang="en">Not intended to be used directly. Use instances of this class instead.</iirds:description>
		<rdfs:comment xml:lang="en">information subject that covers qualitative and quantitative characteristics of technical objects</rdfs:comment>
		<iirds:description xml:lang="en">IRI: required</iirds:description>
	</rdfs:Class>
	<rdfs:Class rdf:about="http://iirds.tekom.de/iirds#TechnicalOverview">
		<rdfs:label xml:lang="de">Technische Übersicht</rdfs:label>
		<rdfs:label xml:lang="en">technical overview</rdfs:label>
		<rdfs:subClassOf rdf:resource="http://iirds.tekom.de/iirds#InformationSubject"/>
		<iirds:description xml:lang="en">Examples are circuit diagrams, flow diagrams, software interface overviews, and pneumatic diagrams.</iirds:description>
		<rdfs:comment xml:lang="en">information subject that covers the technical structure of a product</rdfs:comment>
		<iirds:description xml:lang="en">IRI: required</iirds:description>
	</rdfs:Class>
	<rdfs:Class rdf:about="http://iirds.tekom.de/iirds#Topic">
		<rdfs:label xml:lang="de">Topic</rdfs:label>
		<rdfs:label xml:lang="en">topic</rdfs:label>
		<rdfs:subClassOf rdf:resource="http://iirds.tekom.de/iirds#InformationUnit"/>
		<iirds:description xml:lang="en">The resource of a topic is a file in the iiRDS package.</iirds:description>
		<rdfs:comment xml:lang="en">information unit that covers a single subject</rdfs:comment>
		<iirds:description xml:lang="en">IRI: required</iirds:description>
	</rdfs:Class>
	<rdfs:Class rdf:about="http://iirds.tekom.de/iirds#TopicType">
		<rdfs:label xml:lang="de">Topictyp</rdfs:label>
		<rdfs:label xml:lang="en">topic type</rdfs:label>
		<rdfs:subClassOf rdf:resource="http://iirds.tekom.de/iirds#InformationType"/>
		<iirds:description xml:lang="en">Possible types include task, learning, and concept. Information units that represent topics may have one or more has-topic-type properties that define the topic's information type. Topics without a has-topic-type property are generic topics, with no specific type.</iirds:description>
		<rdfs:comment xml:lang="en">type of information determined according to functional principles</rdfs:comment>
		<iirds:description xml:lang="en">IRI: required</iirds:description>
	</rdfs:Class>
	<rdfs:Class rdf:about="http://iirds.tekom.de/iirds#Troubleshooting">
		<rdfs:label xml:lang="de">Störungsbeseitigung</rdfs:label>
		<rdfs:label xml:lang="en">troubleshooting </rdfs:label>
		<rdfs:subClassOf rdf:resource="http://iirds.tekom.de/iirds#TopicType"/>
		<iirds:description xml:lang="en">Typical troubleshooting topics contain sections with a description of the system's behavior or symptom, the cause for the error, and a remedy for the error.</iirds:description>
		<rdfs:comment xml:lang="en">topic type that provides an explanation for symptoms, diagnosis, and resolution of problems</rdfs:comment>
		<iirds:description xml:lang="en">IRI: required</iirds:description>
	</rdfs:Class>
	<rdfs:Class rdf:about="http://iirds.tekom.de/iirds#Use">
		<rdfs:label xml:lang="de">Nutzung</rdfs:label>
		<rdfs:label xml:lang="en">use</rdfs:label>
		<rdfs:subClassOf rdf:resource="http://iirds.tekom.de/iirds#ProductLifeCyclePhase"/>
		<iirds:description xml:lang="en">Not intended to be used directly. Use the subclasses instead. For lifecycle phases not covered by the iiRDS standard subclasses, define custom subclasses.</iirds:description>
		<rdfs:comment xml:lang="en">product life cycle phase in which the product is supposed to realize its function</rdfs:comment>
		<iirds:description xml:lang="en">IRI: required</iirds:description>
	</rdfs:Class>
	<rdfs:Class rdf:about="http://iirds.tekom.de/iirds#WorkingTime">
		<rdfs:label xml:lang="de">Arbeitszeit</rdfs:label>
		<rdfs:label xml:lang="en">working time</rdfs:label>
		<rdfs:subClassOf rdf:resource="http://iirds.tekom.de/iirds#PlanningTime"/>
		<iirds:description xml:lang="en"/>
		<rdfs:comment xml:lang="en">period of time that is required for conducting a specific task</rdfs:comment>
		<iirds:description xml:lang="en">IRI: optional</iirds:description>
	</rdfs:Class>
	<rdf:Property rdf:about="http://iirds.tekom.de/iirds#dateOfCreation">
		<rdfs:label xml:lang="de">Erstellungsdatum</rdfs:label>
		<rdfs:label xml:lang="en">date of Creation</rdfs:label>
		<rdfs:subPropertyOf rdf:resource="http://purl.org/dc/terms/created"/>
		<rdfs:subPropertyOf rdf:resource="http://iirds.tekom.de/iirds#iirdsAttribute"/>
		<rdfs:domain rdf:resource="http://iirds.tekom.de/iirds#InformationUnit"/>
		<rdfs:range rdf:resource="http://www.w3.org/2001/XMLSchema#dateTimeStamp"/>
		<iirds:description xml:lang="en"/>
		<rdfs:comment xml:lang="en">date of creation of the resource</rdfs:comment>
		<schema:domainIncludes rdf:resource="http://iirds.tekom.de/iirds#InformationUnit"/>
		<schema:rangeIncludes rdf:resource="http://www.w3.org/2001/XMLSchema#dateTimeStamp"/>
		<iirds:description xml:lang="en">Cardinality: http://iirds.tekom.de/iirds#InformationUnit [0..1]</iirds:description>
	</rdf:Property>
	<rdf:Property rdf:about="http://iirds.tekom.de/iirds#dateOfEffect">
		<rdfs:label xml:lang="de">Gültigkeitsbeginn</rdfs:label>
		<rdfs:label xml:lang="en">effective date</rdfs:label>
		<rdfs:subPropertyOf rdf:resource="http://iirds.tekom.de/iirds#iirdsAttribute"/>
		<rdfs:domain rdf:resource="http://iirds.tekom.de/iirds#ContentLifeCycleStatus"/>
		<rdfs:range rdf:resource="http://www.w3.org/2001/XMLSchema#dateTimeStamp"/>
		<iirds:description xml:lang="en"/>
		<rdfs:comment xml:lang="en">date and time on which the given content lifecycle status becomes valid</rdfs:comment>
		<schema:domainIncludes rdf:resource="http://iirds.tekom.de/iirds#ContentLifeCycleStatus"/>
		<schema:rangeIncludes rdf:resource="http://www.w3.org/2001/XMLSchema#dateTimeStamp"/>
		<iirds:description xml:lang="en">Cardinality: http://iirds.tekom.de/iirds#ContentLifeCycleStatus [0..1]</iirds:description>
	</rdf:Property>
	<rdf:Property rdf:about="http://iirds.tekom.de/iirds#dateOfExpiry">
		<rdfs:label xml:lang="de">Auslaufdatum</rdfs:label>
		<rdfs:label xml:lang="en">expiry date</rdfs:label>
		<rdfs:subPropertyOf rdf:resource="http://iirds.tekom.de/iirds#iirdsAttribute"/>
		<rdfs:domain rdf:resource="http://iirds.tekom.de/iirds#ContentLifeCycleStatus"/>
		<rdfs:range rdf:resource="http://www.w3.org/2001/XMLSchema#dateTimeStamp"/>
		<iirds:description xml:lang="en"/>
		<rdfs:comment xml:lang="en">date and time on which the given content lifecycle status becomes invalid</rdfs:comment>
		<schema:domainIncludes rdf:resource="http://iirds.tekom.de/iirds#ContentLifeCycleStatus"/>
		<schema:rangeIncludes rdf:resource="http://www.w3.org/2001/XMLSchema#dateTimeStamp"/>
		<iirds:description xml:lang="en">Cardinality: http://iirds.tekom.de/iirds#ContentLifeCycleStatus [0..1]</iirds:description>
	</rdf:Property>
	<rdf:Property rdf:about="http://iirds.tekom.de/iirds#dateOfLastModification">
		<rdfs:label xml:lang="de">Letztes Änderungsdatum</rdfs:label>
		<rdfs:label xml:lang="en">date of last modification</rdfs:label>
		<rdfs:subPropertyOf rdf:resource="http://iirds.tekom.de/iirds#iirdsAttribute"/>
		<rdfs:range rdf:resource="http://www.w3.org/2001/XMLSchema#dateTimeStamp"/>
		<iirds:description xml:lang="en"/>
		<rdfs:comment xml:lang="en">date and time of an information unit's last change </rdfs:comment>
		<schema:domainIncludes rdf:resource="http://iirds.tekom.de/iirds#InformationUnit"/>
		<schema:rangeIncludes rdf:resource="http://www.w3.org/2001/XMLSchema#dateTimeStamp"/>
		<iirds:description xml:lang="en">Cardinality: http://iirds.tekom.de/iirds#InformationUnit [0..1]</iirds:description>
	</rdf:Property>
	<rdf:Property rdf:about="http://iirds.tekom.de/iirds#dateOfStatus">
		<rdfs:label xml:lang="de">Vergabedatum</rdfs:label>
		<rdfs:label xml:lang="en">status date</rdfs:label>
		<rdfs:subPropertyOf rdf:resource="http://iirds.tekom.de/iirds#iirdsAttribute"/>
		<rdfs:domain rdf:resource="http://iirds.tekom.de/iirds#ContentLifeCycleStatus"/>
		<rdfs:range rdf:resource="http://www.w3.org/2001/XMLSchema#dateTimeStamp"/>
		<iirds:description xml:lang="en"/>
		<rdfs:comment xml:lang="en">date and time of a lifecycle status's last change</rdfs:comment>
		<schema:domainIncludes rdf:resource="http://iirds.tekom.de/iirds#ContentLifeCycleStatus"/>
		<schema:rangeIncludes rdf:resource="http://www.w3.org/2001/XMLSchema#dateTimeStamp"/>
		<iirds:description xml:lang="en">Cardinality: http://iirds.tekom.de/iirds#ContentLifeCycleStatus [0..1]</iirds:description>
	</rdf:Property>
	<rdf:Property rdf:about="http://iirds.tekom.de/iirds#description">
		<rdfs:label xml:lang="de">Beschreibung</rdfs:label>
		<rdfs:label xml:lang="en">description</rdfs:label>
		<rdfs:subPropertyOf rdf:resource="http://purl.org/dc/terms/description"/>
		<rdfs:subPropertyOf rdf:resource="http://iirds.tekom.de/iirds#iirdsAttribute"/>
		<rdfs:range rdf:resource="http://www.w3.org/2000/01/rdf-schema#Literal"/>
		<iirds:description xml:lang="en">Typically a free-text acount of the resource</iirds:description>
		<rdfs:comment xml:lang="en">account on the resource</rdfs:comment>
		<schema:domainIncludes rdf:resource="http://iirds.tekom.de/iirds#iirdsDomainEntity"/>
		<schema:rangeIncludes rdf:resource="http://www.w3.org/2000/01/rdf-schema#Literal"/>
		<iirds:description xml:lang="en">Cardinality: http://iirds.tekom.de/iirds#iirdsDomainEntity [0..*]</iirds:description>
	</rdf:Property>
	<rdf:Property rdf:about="http://iirds.tekom.de/iirds#duration">
		<rdfs:label xml:lang="de">Dauer</rdfs:label>
		<rdfs:label xml:lang="en">duration</rdfs:label>
		<rdfs:subPropertyOf rdf:resource="http://iirds.tekom.de/iirds#iirdsAttribute"/>
		<rdfs:domain rdf:resource="http://iirds.tekom.de/iirds#PlanningTime"/>
		<rdfs:range rdf:resource="http://www.w3.org/2001/XMLSchema#duration"/>
		<iirds:description xml:lang="en"/>
		<rdfs:comment xml:lang="en">span of time</rdfs:comment>
		<schema:domainIncludes rdf:resource="http://iirds.tekom.de/iirds#PlanningTime"/>
		<schema:rangeIncludes rdf:resource="http://www.w3.org/2001/XMLSchema#duration"/>
		<iirds:description xml:lang="en">Cardinality: http://iirds.tekom.de/iirds#PlanningTime [1]</iirds:description>
	</rdf:Property>
	<rdf:Property rdf:about="http://iirds.tekom.de/iirds#format">
		<rdfs:label xml:lang="de">Format</rdfs:label>
		<rdfs:label xml:lang="en">format</rdfs:label>
		<rdfs:subPropertyOf rdf:resource="http://purl.org/dc/terms/format"/>
		<rdfs:subPropertyOf rdf:resource="http://iirds.tekom.de/iirds#iirdsAttribute"/>
		<rdfs:domain rdf:resource="http://iirds.tekom.de/iirds#Rendition"/>
		<rdfs:range rdf:resource="http://www.w3.org/2000/01/rdf-schema#Literal"/>
		<iirds:description xml:lang="en"/>
		<rdfs:comment xml:lang="en">media type of the rendition</rdfs:comment>
		<schema:domainIncludes rdf:resource="http://iirds.tekom.de/iirds#Rendition"/>
		<schema:rangeIncludes rdf:resource="http://www.w3.org/2000/01/rdf-schema#Literal"/>
		<iirds:description xml:lang="en">Cardinality: http://iirds.tekom.de/iirds#Rendition [1]</iirds:description>
	</rdf:Property>
	<rdf:Property rdf:about="http://iirds.tekom.de/iirds#formatRestriction">
		<rdfs:label xml:lang="de">Formateinschränkung</rdfs:label>
		<rdfs:label xml:lang="en">format Restriction</rdfs:label>
		<rdfs:subPropertyOf rdf:resource="http://iirds.tekom.de/iirds#iirdsAttribute"/>
		<rdfs:domain rdf:resource="http://iirds.tekom.de/iirds#Package"/>
		<rdfs:range rdf:resource="http://www.w3.org/2000/01/rdf-schema#Literal"/>
		<iirds:description xml:lang="en">Value "A" means that the package uses a restricted set of media formats ("iiRDS/A").</iirds:description>
		<rdfs:comment xml:lang="en">restriction of media formats allowed in an iiRDS package</rdfs:comment>
		<schema:domainIncludes rdf:resource="http://iirds.tekom.de/iirds#Package"/>
		<schema:rangeIncludes rdf:resource="http://www.w3.org/2000/01/rdf-schema#Literal"/>
		<iirds:description xml:lang="en">Cardinality: http://iirds.tekom.de/iirds#Package [0..1]</iirds:description>
	</rdf:Property>
	<rdf:Property rdf:about="http://iirds.tekom.de/iirds#frequency">
		<rdfs:label xml:lang="de">Wartungsfrequenz</rdfs:label>
		<rdfs:label xml:lang="en">maintenance frequency</rdfs:label>
		<rdfs:subPropertyOf rdf:resource="http://iirds.tekom.de/iirds#iirdsAttribute"/>
		<rdfs:domain rdf:resource="http://iirds.tekom.de/iirds#MaintenanceInterval"/>
		<rdfs:range rdf:resource="http://www.w3.org/2000/01/rdf-schema#Literal"/>
		<iirds:description xml:lang="en"/>
		<rdfs:comment xml:lang="en">intended interval between recurring maintanance tasks</rdfs:comment>
		<iirds:description xml:lang="en">Cardinality: http://iirds.tekom.de/iirds#MaintenanceInterval [1]</iirds:description>
	</rdf:Property>
	<rdf:Property rdf:about="http://iirds.tekom.de/iirds#identifier">
		<rdfs:label xml:lang="de">Bezeichner</rdfs:label>
		<rdfs:label xml:lang="en">identifier</rdfs:label>
		<rdfs:subPropertyOf rdf:resource="http://purl.org/dc/terms/identifier"/>
		<rdfs:subPropertyOf rdf:resource="http://iirds.tekom.de/iirds#iirdsAttribute"/>
		<rdfs:domain rdf:resource="http://iirds.tekom.de/iirds#Identity"/>
		<rdfs:range rdf:resource="http://www.w3.org/2000/01/rdf-schema#Literal"/>
		<iirds:description xml:lang="en">Recommended best practice is to identify the resource by means of a string conforming to a formal identification system.</iirds:description>
		<rdfs:comment xml:lang="en">unique name of the resource within a given domain</rdfs:comment>
		<schema:domainIncludes rdf:resource="http://iirds.tekom.de/iirds#Identity"/>
		<schema:rangeIncludes rdf:resource="http://www.w3.org/2000/01/rdf-schema#Literal"/>
		<iirds:description xml:lang="en">Cardinality: http://iirds.tekom.de/iirds#Identity [1]</iirds:description>
	</rdf:Property>
	<rdf:Property rdf:about="http://iirds.tekom.de/iirds#classificationIdentifier">
		<rdfs:label xml:lang="de">Klassifikationsbezeichner</rdfs:label>
		<rdfs:label xml:lang="en">classification identifier</rdfs:label>
		<rdfs:subPropertyOf rdf:resource="http://iirds.tekom.de/iirds#iirdsAttribute"/>
		<rdfs:domain rdf:resource="http://iirds.tekom.de/iirds#ExternalClassification"/>
		<rdfs:range rdf:resource="http://www.w3.org/2000/01/rdf-schema#Literal"/>
		<iirds:description xml:lang="en">Recommended best practice is to classify the resource by means of a string conforming to a non-IRI identifier in an external classification domain.</iirds:description>
		<rdfs:comment xml:lang="en">classification identifier of the resource within an external classification domain</rdfs:comment>
		<schema:domainIncludes rdf:resource="http://iirds.tekom.de/iirds#ExternalClassification"/>
		<schema:rangeIncludes rdf:resource="http://www.w3.org/2000/01/rdf-schema#Literal"/>
		<iirds:description xml:lang="en">Cardinality: http://iirds.tekom.de/iirds#ExternalClassification [1]</iirds:description>
	</rdf:Property>
	<rdf:Property rdf:about="http://iirds.tekom.de/iirds#classificationVersion">
		<rdfs:label xml:lang="de">Klassifikationsversion</rdfs:label>
		<rdfs:label xml:lang="en">classification version</rdfs:label>
		<rdfs:subPropertyOf rdf:resource="http://iirds.tekom.de/iirds#iirdsAttribute"/>
		<rdfs:domain rdf:resource="http://iirds.tekom.de/iirds#ExternalClassification"/>
		<rdfs:range rdf:resource="http://www.w3.org/2000/01/rdf-schema#Literal"/>
		<iirds:description xml:lang="en">Recommended best practice is to use the version or release date of the external classification.</iirds:description>
		<rdfs:comment xml:lang="en">version of the external classification</rdfs:comment>
		<schema:domainIncludes rdf:resource="http://iirds.tekom.de/iirds#ExternalClassification"/>
		<schema:rangeIncludes rdf:resource="http://www.w3.org/2000/01/rdf-schema#Literal"/>
		<iirds:description xml:lang="en">Cardinality: http://iirds.tekom.de/iirds#ExternalClassification [0..1]</iirds:description>
	</rdf:Property>
	<rdf:Property rdf:about="http://iirds.tekom.de/iirds#iirdsAttribute">
		<rdfs:label xml:lang="de">iirdsAttribute</rdfs:label>
		<rdfs:label xml:lang="en">iirdsAttribute</rdfs:label>
		<rdfs:range rdf:resource="http://www.w3.org/2000/01/rdf-schema#Literal"/>
		<iirds:description xml:lang="en">Not intended to be used directly. Use the subclasses instead.</iirds:description>
		<rdfs:comment xml:lang="en">property with a literal value</rdfs:comment>
		<schema:domainIncludes rdf:resource="http://iirds.tekom.de/iirds#iirdsDomainEntity"/>
		<schema:rangeIncludes rdf:resource="http://www.w3.org/2000/01/rdf-schema#Literal"/>
	</rdf:Property>
	<rdf:Property rdf:about="http://iirds.tekom.de/iirds#iiRDSVersion">
		<rdfs:label xml:lang="de">iiRDS Version</rdfs:label>
		<rdfs:label xml:lang="en">iiRDS version</rdfs:label>
		<rdfs:subPropertyOf rdf:resource="http://iirds.tekom.de/iirds#iirdsAttribute"/>
		<rdfs:domain rdf:resource="http://iirds.tekom.de/iirds#Package"/>
		<rdfs:range rdf:resource="http://www.w3.org/2000/01/rdf-schema#Literal"/>
		<iirds:description xml:lang="en">Current version is 1.0.</iirds:description>
		<rdfs:comment xml:lang="en">iiRDS version with which the iiRDS package complies</rdfs:comment>
		<schema:domainIncludes rdf:resource="http://iirds.tekom.de/iirds#Package"/>
		<schema:rangeIncludes rdf:resource="http://www.w3.org/2000/01/rdf-schema#Literal"/>
		<iirds:description xml:lang="en">Cardinality: http://iirds.tekom.de/iirds#Package [1]</iirds:description>
	</rdf:Property>
	<rdf:Property rdf:about="http://iirds.tekom.de/iirds#language">
		<rdfs:label xml:lang="de">Sprache</rdfs:label>
		<rdfs:label xml:lang="en">language</rdfs:label>
		<rdfs:subPropertyOf rdf:resource="http://purl.org/dc/terms/language"/>
		<rdfs:subPropertyOf rdf:resource="http://iirds.tekom.de/iirds#iirdsAttribute"/>
		<rdfs:domain rdf:resource="http://iirds.tekom.de/iirds#InformationUnit"/>
		<rdfs:range rdf:resource="http://www.w3.org/2000/01/rdf-schema#Literal"/>
		<iirds:description xml:lang="en">Controlled vocabulary according to RFC 4646.</iirds:description>
		<rdfs:comment xml:lang="en">identifier of the content's language</rdfs:comment>
		<schema:domainIncludes rdf:resource="http://iirds.tekom.de/iirds#InformationUnit"/>
		<schema:rangeIncludes rdf:resource="http://www.w3.org/2000/01/rdf-schema#Literal"/>
		<iirds:description xml:lang="en">Cardinality: http://iirds.tekom.de/iirds#InformationUnit [0..*]</iirds:description>
	</rdf:Property>
	<rdf:Property rdf:about="http://iirds.tekom.de/iirds#revision">
		<rdfs:label xml:lang="de">Revision</rdfs:label>
		<rdfs:label xml:lang="en">revision</rdfs:label>
		<rdfs:subPropertyOf rdf:resource="http://iirds.tekom.de/iirds#iirdsAttribute"/>
		<rdfs:domain rdf:resource="http://iirds.tekom.de/iirds#InformationUnit"/>
		<rdfs:range rdf:resource="http://www.w3.org/2000/01/rdf-schema#Literal"/>
		<iirds:description xml:lang="en"/>
		<rdfs:comment xml:lang="en">version of an information unit</rdfs:comment>
		<schema:domainIncludes rdf:resource="http://iirds.tekom.de/iirds#InformationUnit"/>
		<schema:rangeIncludes rdf:resource="http://www.w3.org/2000/01/rdf-schema#Literal"/>
		<iirds:description xml:lang="en">Cardinality: http://iirds.tekom.de/iirds#InformationUnit [0..1]</iirds:description>
	</rdf:Property>
	<rdf:Property rdf:about="http://iirds.tekom.de/iirds#rights">
		<rdfs:label xml:lang="de">Rechte</rdfs:label>
		<rdfs:label xml:lang="en">rights</rdfs:label>
		<rdfs:subPropertyOf rdf:resource="http://purl.org/dc/elements/1.1/rights"/>
		<rdfs:subPropertyOf rdf:resource="http://iirds.tekom.de/iirds#iirdsAttribute"/>
		<rdfs:domain rdf:resource="http://iirds.tekom.de/iirds#InformationUnit"/>
		<rdfs:range rdf:resource="http://www.w3.org/2000/01/rdf-schema#Literal"/>
		<iirds:description xml:lang="en"/>
		<rdfs:comment xml:lang="en">declaration of specific rights regarding the usage of the information</rdfs:comment>
		<schema:domainIncludes rdf:resource="http://iirds.tekom.de/iirds#InformationUnit"/>
		<schema:rangeIncludes rdf:resource="http://www.w3.org/2000/01/rdf-schema#Literal"/>
		<iirds:description xml:lang="en">Cardinality: http://iirds.tekom.de/iirds#InformationUnit [0..*]</iirds:description>
	</rdf:Property>
	<rdf:Property rdf:about="http://iirds.tekom.de/iirds#statusComment">
		<rdfs:label xml:lang="de">Kommentar zum Status</rdfs:label>
		<rdfs:label xml:lang="en">status comment</rdfs:label>
		<rdfs:subPropertyOf rdf:resource="http://iirds.tekom.de/iirds#iirdsAttribute"/>
		<rdfs:domain rdf:resource="http://iirds.tekom.de/iirds#ContentLifeCycleStatus"/>
		<rdfs:range rdf:resource="http://www.w3.org/2000/01/rdf-schema#Literal"/>
		<iirds:description xml:lang="en"/>
		<rdfs:comment xml:lang="en">note on a content lifecycle status</rdfs:comment>
		<schema:domainIncludes rdf:resource="http://iirds.tekom.de/iirds#ContentLifeCycleStatus"/>
		<schema:rangeIncludes rdf:resource="http://www.w3.org/2000/01/rdf-schema#Literal"/>
		<iirds:description xml:lang="en">Cardinality: http://iirds.tekom.de/iirds#ContentLifeCycleStatus [0..*]</iirds:description>
	</rdf:Property>
	<rdf:Property rdf:about="http://iirds.tekom.de/iirds#source">
		<rdfs:label xml:lang="de">Quelle</rdfs:label>
		<rdfs:label xml:lang="en">source</rdfs:label>
		<rdfs:subPropertyOf rdf:resource="http://iirds.tekom.de/iirds#iirdsAttribute"/>
		<rdfs:domain rdf:resource="http://iirds.tekom.de/iirds#Rendition"/>
		<rdfs:range rdf:resource="http://www.w3.org/2000/01/rdf-schema#Literal"/>
		<iirds:description xml:lang="de">The path is relative to the root directory of the package, e.g., "content/overview.html".</iirds:description>
		<rdfs:comment xml:lang="en">relative path of a file in an iiRDS package that contains the content of a rendition</rdfs:comment>
		<schema:domainIncludes rdf:resource="http://iirds.tekom.de/iirds#Rendition"/>
		<schema:rangeIncludes rdf:resource="http://www.w3.org/2000/01/rdf-schema#Literal"/>
		<iirds:description xml:lang="en">Cardinality: http://iirds.tekom.de/iirds#Rendition [1]</iirds:description>
	</rdf:Property>
	<rdf:Property rdf:about="http://iirds.tekom.de/iirds#synonym">
		<rdfs:label xml:lang="de">Synonym</rdfs:label>
		<rdfs:label xml:lang="en">synonym</rdfs:label>
		<rdfs:subPropertyOf rdf:resource="http://iirds.tekom.de/iirds#iirdsAttribute"/>
		<rdfs:domain rdf:resource="http://iirds.tekom.de/iirds#iirdsDomainEntity"/>
		<rdfs:range rdf:resource="http://www.w3.org/2000/01/rdf-schema#Literal"/>
		<iirds:description xml:lang="en"/>
		<rdfs:comment xml:lang="en">word or phrase that means exactly or nearly the same as another word or phrase in the same language</rdfs:comment>
		<schema:domainIncludes rdf:resource="http://iirds.tekom.de/iirds#iirdsDomainEntity"/>
		<schema:rangeIncludes rdf:resource="http://www.w3.org/2000/01/rdf-schema#Literal"/>
		<iirds:description xml:lang="en">Cardinality: http://iirds.tekom.de/iirds#iirdsDomainEntity [0..*]</iirds:description>
	</rdf:Property>
	<rdf:Property rdf:about="http://iirds.tekom.de/iirds#title">
		<rdfs:label xml:lang="de">Titel</rdfs:label>
		<rdfs:label xml:lang="en">title</rdfs:label>
		<rdfs:subPropertyOf rdf:resource="http://purl.org/dc/terms/title"/>
		<rdfs:subPropertyOf rdf:resource="http://iirds.tekom.de/iirds#iirdsAttribute"/>
		<rdfs:domain rdf:resource="http://iirds.tekom.de/iirds#InformationUnit"/>
		<rdfs:range rdf:resource="http://www.w3.org/2000/01/rdf-schema#Literal"/>
		<iirds:description xml:lang="en">Typically, a title will be a name by which the information unit is formally known.</iirds:description>
		<rdfs:comment xml:lang="en">name of the information unit</rdfs:comment>
		<schema:domainIncludes rdf:resource="http://iirds.tekom.de/iirds#InformationUnit"/>
		<schema:rangeIncludes rdf:resource="http://www.w3.org/2000/01/rdf-schema#Literal"/>
		<iirds:description xml:lang="en">Cardinality: http://iirds.tekom.de/iirds#InformationUnit [0..1]</iirds:description>
	</rdf:Property>
	<rdf:Property rdf:about="http://iirds.tekom.de/iirds#is-applicable-for-document-type">
		<rdfs:label xml:lang="de">geeignet für Dokumentart</rdfs:label>
		<rdfs:label xml:lang="en">applicable for document type</rdfs:label>
		<rdfs:subPropertyOf rdf:resource="http://iirds.tekom.de/iirds#has-information-type"/>
		<rdfs:domain rdf:resource="http://iirds.tekom.de/iirds#InformationUnit"/>
		<rdfs:range rdf:resource="http://iirds.tekom.de/iirds#DocumentType"/>
		<iirds:description xml:lang="en">Example: topics that are suitable for the installation instructions.</iirds:description>
		<rdfs:comment xml:lang="en">information unit's property that references a document type the information unit is suitable for</rdfs:comment>
		<schema:domainIncludes rdf:resource="http://iirds.tekom.de/iirds#InformationUnit"/>
		<schema:rangeIncludes rdf:resource="http://iirds.tekom.de/iirds#DocumentType"/>
		<iirds:description xml:lang="en">Cardinality: http://iirds.tekom.de/iirds#InformationUnit [0..*]</iirds:description>
	</rdf:Property>
	<rdf:Property rdf:about="http://iirds.tekom.de/iirds#has-abstract">
		<rdfs:label xml:lang="de">hat Zusammenfassung</rdfs:label>
		<rdfs:label xml:lang="en">has abstract</rdfs:label>
		<rdfs:subPropertyOf rdf:resource="http://purl.org/dc/terms/abstract"/>
		<rdfs:subPropertyOf rdf:resource="http://iirds.tekom.de/iirds#iirdsRelationConcept"/>
		<rdfs:domain rdf:resource="http://iirds.tekom.de/iirds#InformationUnit"/>
		<iirds:description xml:lang="en"/>
		<rdfs:comment xml:lang="en">summary of the resource</rdfs:comment>
		<schema:domainIncludes rdf:resource="http://iirds.tekom.de/iirds#InformationUnit"/>
		<iirds:description xml:lang="en">Cardinality: http://iirds.tekom.de/iirds#InformationUnit [0..1]</iirds:description>
	</rdf:Property>
	<rdf:Property rdf:about="http://iirds.tekom.de/iirds#has-component">
		<rdfs:label xml:lang="de">hat Komponente</rdfs:label>
		<rdfs:label xml:lang="en">has component</rdfs:label>
		<rdfs:subPropertyOf rdf:resource="http://iirds.tekom.de/iirds#iirdsRelationConcept"/>
		<rdfs:domain rdf:resource="http://iirds.tekom.de/iirds#Component"/>
		<rdfs:range rdf:resource="http://iirds.tekom.de/iirds#Component"/>
		<iirds:description xml:lang="en"/>
		<rdfs:comment xml:lang="en">property that references a component</rdfs:comment>
		<schema:domainIncludes rdf:resource="http://iirds.tekom.de/iirds#Component"/>
		<schema:rangeIncludes rdf:resource="http://iirds.tekom.de/iirds#Component"/>
		<iirds:description xml:lang="en">Cardinality: http://iirds.tekom.de/iirds#Component [0..*]</iirds:description>
	</rdf:Property>
	<rdf:Property rdf:about="http://iirds.tekom.de/iirds#has-content-lifecycle-status">
		<rdfs:label xml:lang="de">hat Beziehung zu Bearbeitungsstatus</rdfs:label>
		<rdfs:label xml:lang="en">relates to content lifecycle status</rdfs:label>
		<rdfs:subPropertyOf rdf:resource="http://iirds.tekom.de/iirds#relates-to-administrative-metadata"/>
		<rdfs:domain rdf:resource="http://iirds.tekom.de/iirds#InformationUnit"/>
		<rdfs:range rdf:resource="http://iirds.tekom.de/iirds#ContentLifeCycleStatus"/>
		<iirds:description xml:lang="en"/>
		<rdfs:comment xml:lang="en">information unit's property that references its content lifecycle status</rdfs:comment>
		<schema:domainIncludes rdf:resource="http://iirds.tekom.de/iirds#InformationUnit"/>
		<schema:rangeIncludes rdf:resource="http://iirds.tekom.de/iirds#ContentLifeCycleStatus"/>
		<iirds:description xml:lang="en">Cardinality: http://iirds.tekom.de/iirds#InformationUnit [0..*]</iirds:description>
	</rdf:Property>
	<rdf:Property rdf:about="http://iirds.tekom.de/iirds#has-content-lifecycle-status-value">
		<rdfs:label xml:lang="de">hat Statuswert</rdfs:label>
		<rdfs:label xml:lang="en">has status value</rdfs:label>
		<rdfs:subPropertyOf rdf:resource="http://iirds.tekom.de/iirds#iirdsRelationConcept"/>
		<rdfs:domain rdf:resource="http://iirds.tekom.de/iirds#ContentLifeCycleStatus"/>
		<rdfs:range rdf:resource="http://iirds.tekom.de/iirds#ContentLifeCycleStatusValue"/>
		<iirds:description xml:lang="en"/>
		<rdfs:comment xml:lang="en">content lifecycle status's property that references its value</rdfs:comment>
		<schema:domainIncludes rdf:resource="http://iirds.tekom.de/iirds#ContentLifeCycleStatus"/>
		<schema:rangeIncludes rdf:resource="http://iirds.tekom.de/iirds#ContentLifeCycleStatusValue"/>
		<iirds:description xml:lang="en">Cardinality: http://iirds.tekom.de/iirds#ContentLifeCycleStatus [1]</iirds:description>
	</rdf:Property>
	<rdf:Property rdf:about="http://iirds.tekom.de/iirds#has-directory-structure-type">
		<rdfs:label xml:lang="de">hat Verzeichnisstrukturtyp</rdfs:label>
		<rdfs:label xml:lang="en">has directory structure type</rdfs:label>
		<rdfs:subPropertyOf rdf:resource="http://iirds.tekom.de/iirds#iirdsRelationConcept"/>
		<rdfs:domain rdf:resource="http://iirds.tekom.de/iirds#DirectoryNode"/>
		<rdfs:range rdf:resource="http://iirds.tekom.de/iirds#DirectoryNodeType"/>
		<iirds:description xml:lang="en"/>
		<rdfs:comment xml:lang="en">directory node's property that references its node type</rdfs:comment>
		<schema:domainIncludes rdf:resource="http://iirds.tekom.de/iirds#DirectoryNode"/>
		<schema:rangeIncludes rdf:resource="http://iirds.tekom.de/iirds#DirectoryNodeType"/>
		<iirds:description xml:lang="en">Cardinality: http://iirds.tekom.de/iirds#DirectoryNode [0..1]</iirds:description>
	</rdf:Property>
	<rdf:Property rdf:about="http://iirds.tekom.de/iirds#has-document-type">
		<rdfs:label xml:lang="de">hat Dokumentart</rdfs:label>
		<rdfs:label xml:lang="en">has document type</rdfs:label>
		<rdfs:subPropertyOf rdf:resource="http://iirds.tekom.de/iirds#has-information-type"/>
		<rdfs:domain rdf:resource="http://iirds.tekom.de/iirds#Document"/>
		<rdfs:range rdf:resource="http://iirds.tekom.de/iirds#DocumentType"/>
		<iirds:description xml:lang="en">Documents have one or more document types. Documents without document types are unspecific documents.</iirds:description>
		<rdfs:comment xml:lang="en">document's property that references its document type</rdfs:comment>
		<schema:domainIncludes rdf:resource="http://iirds.tekom.de/iirds#Document"/>
		<schema:rangeIncludes rdf:resource="http://iirds.tekom.de/iirds#DocumentType"/>
		<iirds:description xml:lang="en">Cardinality: http://iirds.tekom.de/iirds#Document [1..*]</iirds:description>
	</rdf:Property>
	<rdf:Property rdf:about="http://iirds.tekom.de/iirds#has-end-selector">
		<rdfs:label xml:lang="de">hat Endselektor</rdfs:label>
		<rdfs:label xml:lang="en">has end selector</rdfs:label>
		<rdfs:subPropertyOf rdf:resource="http://iirds.tekom.de/iirds#has-selector"/>
		<rdfs:domain rdf:resource="http://iirds.tekom.de/iirds#RangeSelector"/>
		<rdfs:range rdf:resource="http://iirds.tekom.de/iirds#FragmentSelector"/>
		<iirds:description xml:lang="en">A range selector must reference one start and one end selector.</iirds:description>
		<rdfs:comment xml:lang="en">range selector's property that references the end of its  range</rdfs:comment>
		<schema:domainIncludes rdf:resource="http://iirds.tekom.de/iirds#RangeSelector"/>
		<schema:rangeIncludes rdf:resource="http://iirds.tekom.de/iirds#FragmentSelector"/>
		<iirds:description xml:lang="en">Cardinality: http://iirds.tekom.de/iirds#RangeSelector [1]</iirds:description>
	</rdf:Property>
	<rdf:Property rdf:about="http://iirds.tekom.de/iirds#has-event-code">
		<rdfs:label xml:lang="de">hat Ereigniscode</rdfs:label>
		<rdfs:label xml:lang="en">has event code</rdfs:label>
		<rdfs:subPropertyOf rdf:resource="http://iirds.tekom.de/iirds#iirdsRelationConcept"/>
		<rdfs:domain rdf:resource="http://iirds.tekom.de/iirds#Event"/>
		<iirds:description xml:lang="en"/>
		<rdfs:comment xml:lang="en">property to identify an event</rdfs:comment>
		<schema:domainIncludes rdf:resource="http://iirds.tekom.de/iirds#Event"/>
		<iirds:description xml:lang="en">Cardinality: http://iirds.tekom.de/iirds#Event [0..1]</iirds:description>
	</rdf:Property>
	<rdf:Property rdf:about="http://iirds.tekom.de/iirds#has-event-type">
		<rdfs:label xml:lang="de">hat Ereignistyp</rdfs:label>
		<rdfs:label xml:lang="en">has event type</rdfs:label>
		<rdfs:subPropertyOf rdf:resource="http://iirds.tekom.de/iirds#iirdsRelationConcept"/>
		<rdfs:domain rdf:resource="http://iirds.tekom.de/iirds#Event"/>
		<iirds:description xml:lang="en"/>
		<rdfs:comment xml:lang="en">event's property that references its type</rdfs:comment>
		<schema:domainIncludes rdf:resource="http://iirds.tekom.de/iirds#Event"/>
		<iirds:description xml:lang="en">Cardinality: http://iirds.tekom.de/iirds#Event [0..1]</iirds:description>
	</rdf:Property>
	<rdf:Property rdf:about="http://iirds.tekom.de/iirds#has-first-child">
		<rdfs:label xml:lang="de">hat als erstes Kindelement</rdfs:label>
		<rdfs:label xml:lang="en">has first child</rdfs:label>
		<rdfs:subPropertyOf rdf:resource="http://iirds.tekom.de/iirds#iirdsRelationConcept"/>
		<rdfs:domain rdf:resource="http://iirds.tekom.de/iirds#DirectoryNode"/>
		<rdfs:range rdf:resource="http://iirds.tekom.de/iirds#DirectoryNode"/>
		<iirds:description xml:lang="en"/>
		<rdfs:comment xml:lang="en">directory node's property that references the first directory node on the next subordinate level in a directory structure</rdfs:comment>
		<schema:domainIncludes rdf:resource="http://iirds.tekom.de/iirds#DirectoryNode"/>
		<schema:rangeIncludes rdf:resource="http://iirds.tekom.de/iirds#DirectoryNode"/>
		<iirds:description xml:lang="en">Cardinality: http://iirds.tekom.de/iirds#DirectoryNode [0..1]</iirds:description>
	</rdf:Property>
	<rdf:Property rdf:about="http://iirds.tekom.de/iirds#has-identity">
		<rdfs:label xml:lang="de">hat komplexen Identifier</rdfs:label>
		<rdfs:label xml:lang="en">has complex identifier</rdfs:label>
		<rdfs:subPropertyOf rdf:resource="http://iirds.tekom.de/iirds#relates-to-administrative-metadata"/>
		<rdfs:range rdf:resource="http://iirds.tekom.de/iirds#Identity"/>
		<iirds:description xml:lang="en"/>
		<rdfs:comment xml:lang="en">iiRDS resource's property that references an identifier</rdfs:comment>
		<schema:domainIncludes rdf:resource="http://iirds.tekom.de/iirds#Component"/>
		<schema:domainIncludes rdf:resource="http://iirds.tekom.de/iirds#InformationObject"/>
		<schema:domainIncludes rdf:resource="http://iirds.tekom.de/iirds#InformationUnit"/>
		<schema:domainIncludes rdf:resource="http://iirds.tekom.de/iirds#ProductVariant"/>
		<schema:domainIncludes rdf:resource="http://iirds.tekom.de/iirds#Rendition"/>
		<schema:rangeIncludes rdf:resource="http://iirds.tekom.de/iirds#Identity"/>
		<iirds:description xml:lang="en">Cardinality: http://iirds.tekom.de/iirds#Component [0..*]</iirds:description>
		<iirds:description xml:lang="en">Cardinality: http://iirds.tekom.de/iirds#InformationObject [0..*]</iirds:description>
		<iirds:description xml:lang="en">Cardinality: http://iirds.tekom.de/iirds#InformationUnit [0..*]</iirds:description>
		<iirds:description xml:lang="en">Cardinality: http://iirds.tekom.de/iirds#ProductVariant [0..*]</iirds:description>
		<iirds:description xml:lang="en">Cardinality: http://iirds.tekom.de/iirds#Rendition [0..*]</iirds:description>
	</rdf:Property>
	<rdf:Property rdf:about="http://iirds.tekom.de/iirds#has-identity-domain">
		<rdfs:label xml:lang="de">hat Identifier-Domain</rdfs:label>
		<rdfs:label xml:lang="en">has identifier domain</rdfs:label>
		<rdfs:subPropertyOf rdf:resource="http://iirds.tekom.de/iirds#iirdsRelationConcept"/>
		<rdfs:domain rdf:resource="http://iirds.tekom.de/iirds#Identity"/>
		<rdfs:range rdf:resource="http://iirds.tekom.de/iirds#IdentityDomain"/>
		<iirds:description xml:lang="en"/>
		<rdfs:comment xml:lang="en">identifier's property that references the domain in which it is unique</rdfs:comment>
		<schema:domainIncludes rdf:resource="http://iirds.tekom.de/iirds#Identity"/>
		<schema:rangeIncludes rdf:resource="http://iirds.tekom.de/iirds#IdentityDomain"/>
		<iirds:description xml:lang="en">Cardinality: http://iirds.tekom.de/iirds#Identity [1]</iirds:description>
	</rdf:Property>
	<rdf:Property rdf:about="http://iirds.tekom.de/iirds#has-identity-type">
		<rdfs:label xml:lang="de">hat Identifier-Typ</rdfs:label>
		<rdfs:label xml:lang="en">has identifier type</rdfs:label>
		<rdfs:subPropertyOf rdf:resource="http://iirds.tekom.de/iirds#iirdsRelationConcept"/>
		<rdfs:domain rdf:resource="http://iirds.tekom.de/iirds#IdentityDomain"/>
		<rdfs:range rdf:resource="http://iirds.tekom.de/iirds#IdentityType"/>
		<iirds:description xml:lang="en"/>
		<rdfs:comment xml:lang="en">identity domain's property that references its identifier type</rdfs:comment>
		<schema:domainIncludes rdf:resource="http://iirds.tekom.de/iirds#IdentityDomain"/>
		<schema:rangeIncludes rdf:resource="http://iirds.tekom.de/iirds#IdentityType"/>
		<iirds:description xml:lang="en">Cardinality: http://iirds.tekom.de/iirds#IdentityDomain [0..1]</iirds:description>
	</rdf:Property>
	<rdf:Property rdf:about="http://iirds.tekom.de/iirds#has-classification-domain">
		<rdfs:label xml:lang="de">hat Klassifikations-Domain</rdfs:label>
		<rdfs:label xml:lang="en">has classification domain</rdfs:label>
		<rdfs:subPropertyOf rdf:resource="http://iirds.tekom.de/iirds#iirdsRelationConcept"/>
		<rdfs:domain rdf:resource="http://iirds.tekom.de/iirds#ExternalClassification"/>
		<rdfs:range rdf:resource="http://iirds.tekom.de/iirds#ClassificationDomain"/>
		<iirds:description xml:lang="en"/>
		<rdfs:comment xml:lang="en">references the domain that a classification refers to</rdfs:comment>
		<schema:domainIncludes rdf:resource="http://iirds.tekom.de/iirds#ExternalClassification"/>
		<schema:rangeIncludes rdf:resource="http://iirds.tekom.de/iirds#ClassificationDomain"/>
		<iirds:description xml:lang="en">Cardinality: http://iirds.tekom.de/iirds#ExternalClassification [1]</iirds:description>
	</rdf:Property>
	<rdf:Property rdf:about="http://iirds.tekom.de/iirds#has-external-classification">
		<rdfs:label xml:lang="de">hat externe Klassifikation</rdfs:label>
		<rdfs:label xml:lang="en">has external classification</rdfs:label>
		<rdfs:subPropertyOf rdf:resource="http://iirds.tekom.de/iirds#relates-to-administrative-metadata"/>
		<rdfs:range rdf:resource="http://iirds.tekom.de/iirds#ExternalClassification"/>
		<iirds:description xml:lang="en"/>
		<rdfs:comment xml:lang="en">references an external classification</rdfs:comment>
		<schema:domainIncludes rdf:resource="http://iirds.tekom.de/iirds#Component"/>
		<schema:domainIncludes rdf:resource="http://iirds.tekom.de/iirds#InformationUnit"/>
		<schema:domainIncludes rdf:resource="http://iirds.tekom.de/iirds#ProductVariant"/>
		<schema:domainIncludes rdf:resource="http://iirds.tekom.de/iirds#ProductFeature"/>
		<schema:rangeIncludes rdf:resource="http://iirds.tekom.de/iirds#ExternalClassification"/>
		<iirds:description xml:lang="en">Cardinality: http://iirds.tekom.de/iirds#Component [0..*]</iirds:description>
		<iirds:description xml:lang="en">Cardinality: http://iirds.tekom.de/iirds#InformationUnit [0..*]</iirds:description>
		<iirds:description xml:lang="en">Cardinality: http://iirds.tekom.de/iirds#ProductVariant [0..*]</iirds:description>
		<iirds:description xml:lang="en">Cardinality: http://iirds.tekom.de/iirds#ProductFeature [0..*]</iirds:description>
	</rdf:Property>
	<rdf:Property rdf:about="http://iirds.tekom.de/iirds#has-classification-type">
		<rdfs:label xml:lang="de">hat Klassifikations-Typ</rdfs:label>
		<rdfs:label xml:lang="en">has classification type</rdfs:label>
		<rdfs:subPropertyOf rdf:resource="http://iirds.tekom.de/iirds#iirdsRelationConcept"/>
		<rdfs:domain rdf:resource="http://iirds.tekom.de/iirds#ClassificationDomain"/>
		<rdfs:range rdf:resource="http://iirds.tekom.de/iirds#ClassificationType"/>
		<rdfs:comment xml:lang="en">type of the classification or the class name</rdfs:comment>
		<schema:domainIncludes rdf:resource="http://iirds.tekom.de/iirds#ClassificationDomain"/>
		<schema:rangeIncludes rdf:resource="http://iirds.tekom.de/iirds#ClassificationType"/>
		<iirds:description xml:lang="en">Cardinality: http://iirds.tekom.de/iirds#ClassificationDomain [0..1]</iirds:description>
	</rdf:Property>
	<rdf:Property rdf:about="http://iirds.tekom.de/iirds#has-information-type">
		<rdfs:label xml:lang="de">hat Informationsart</rdfs:label>
		<rdfs:label xml:lang="en">has information type</rdfs:label>
		<rdfs:subPropertyOf rdf:resource="http://iirds.tekom.de/iirds#iirdsRelationConcept"/>
		<rdfs:domain rdf:resource="http://iirds.tekom.de/iirds#InformationUnit"/>
		<rdfs:range rdf:resource="http://iirds.tekom.de/iirds#InformationType"/>
		<iirds:description xml:lang="en">Not intended to be used directly. Use the child properties instead, such as has-document-type for documents and has-topic-type for topics.</iirds:description>
		<rdfs:comment xml:lang="en">information unit's property that references its nature or subject</rdfs:comment>
		<schema:domainIncludes rdf:resource="http://iirds.tekom.de/iirds#InformationUnit"/>
		<schema:rangeIncludes rdf:resource="http://iirds.tekom.de/iirds#InformationType"/>
		<iirds:description xml:lang="en">Cardinality: http://iirds.tekom.de/iirds#InformationUnit [0..*]</iirds:description>
	</rdf:Property>
	<rdf:Property rdf:about="http://iirds.tekom.de/iirds#has-next-sibling">
		<rdfs:label xml:lang="de">hat als nächstes Element</rdfs:label>
		<rdfs:label xml:lang="en">has next sibling</rdfs:label>
		<rdfs:subPropertyOf rdf:resource="http://iirds.tekom.de/iirds#iirdsRelationConcept"/>
		<rdfs:domain rdf:resource="http://iirds.tekom.de/iirds#DirectoryNode"/>
		<rdfs:range rdf:resource="http://iirds.tekom.de/iirds#DirectoryNode"/>
		<iirds:description xml:lang="en"/>
		<rdfs:comment xml:lang="en">directory node's property that references the following directory node on the same hierarchy level in a directory structure</rdfs:comment>
		<schema:domainIncludes rdf:resource="http://iirds.tekom.de/iirds#DirectoryNode"/>
		<schema:rangeIncludes rdf:resource="http://iirds.tekom.de/iirds#DirectoryNode"/>
		<iirds:description xml:lang="en">Cardinality: http://iirds.tekom.de/iirds#DirectoryNode [0..1]</iirds:description>
	</rdf:Property>
	<rdf:Property rdf:about="http://iirds.tekom.de/iirds#has-party-role">
		<rdfs:label xml:lang="de">hat administrative Rolle</rdfs:label>
		<rdfs:label xml:lang="en">has administrative role</rdfs:label>
		<rdfs:subPropertyOf rdf:resource="http://iirds.tekom.de/iirds#iirdsRelationConcept"/>
		<rdfs:domain rdf:resource="http://iirds.tekom.de/iirds#Party"/>
		<rdfs:range rdf:resource="http://iirds.tekom.de/iirds#PartyRole"/>
		<iirds:description xml:lang="en"/>
		<rdfs:comment xml:lang="en">party's property that references its role</rdfs:comment>
		<rdfs:comment xml:lang="de"/>
		<schema:domainIncludes rdf:resource="http://iirds.tekom.de/iirds#Party"/>
		<schema:rangeIncludes rdf:resource="http://iirds.tekom.de/iirds#PartyRole"/>
		<iirds:description xml:lang="en">Cardinality: http://iirds.tekom.de/iirds#Party [0..1]</iirds:description>
	</rdf:Property>
	<rdf:Property rdf:about="http://iirds.tekom.de/iirds#has-planning-time">
		<rdfs:label xml:lang="de">hat Zeit</rdfs:label>
		<rdfs:label xml:lang="en">has time</rdfs:label>
		<rdfs:subPropertyOf rdf:resource="http://iirds.tekom.de/iirds#relates-to-functional-metadata"/>
		<rdfs:domain rdf:resource="http://iirds.tekom.de/iirds#InformationUnit"/>
		<rdfs:range rdf:resource="http://iirds.tekom.de/iirds#PlanningTime"/>
		<iirds:description xml:lang="en"/>
		<rdfs:comment xml:lang="en">information unit's property that references the planning time</rdfs:comment>
		<schema:domainIncludes rdf:resource="http://iirds.tekom.de/iirds#InformationUnit"/>
		<schema:rangeIncludes rdf:resource="http://iirds.tekom.de/iirds#PlanningTime"/>
		<iirds:description xml:lang="en">Cardinality: http://iirds.tekom.de/iirds#InformationUnit [0..*]</iirds:description>
	</rdf:Property>
	<rdf:Property rdf:about="http://iirds.tekom.de/iirds#has-rendition">
		<rdfs:label xml:lang="de">hat Inhaltsausprägung</rdfs:label>
		<rdfs:label xml:lang="en">has rendition</rdfs:label>
		<rdfs:subPropertyOf rdf:resource="http://iirds.tekom.de/iirds#iirdsRelationConcept"/>
		<rdfs:domain rdf:resource="http://iirds.tekom.de/iirds#InformationUnit"/>
		<rdfs:range rdf:resource="http://iirds.tekom.de/iirds#Rendition"/>
		<iirds:description xml:lang="en"/>
		<rdfs:comment xml:lang="en">information unit's property that references its rendition</rdfs:comment>
		<schema:domainIncludes rdf:resource="http://iirds.tekom.de/iirds#InformationUnit"/>
		<schema:rangeIncludes rdf:resource="http://iirds.tekom.de/iirds#Rendition"/>
		<iirds:description xml:lang="en">Cardinality: http://iirds.tekom.de/iirds#InformationUnit [0..*]</iirds:description>
	</rdf:Property>
	<rdf:Property rdf:about="http://iirds.tekom.de/iirds#has-selector">
		<rdfs:label xml:lang="de">hat Selektor</rdfs:label>
		<rdfs:label xml:lang="en">has selector</rdfs:label>
		<rdfs:subPropertyOf rdf:resource="http://iirds.tekom.de/iirds#iirdsRelationConcept"/>
		<rdfs:range rdf:resource="http://iirds.tekom.de/iirds#Selector"/>
		<iirds:description xml:lang="en"/>
		<rdfs:comment xml:lang="en">rendition's property that references a selector</rdfs:comment>
		<schema:domainIncludes rdf:resource="http://iirds.tekom.de/iirds#Rendition"/>
		<schema:rangeIncludes rdf:resource="http://iirds.tekom.de/iirds#Selector"/>
		<iirds:description xml:lang="en">Cardinality: http://iirds.tekom.de/iirds#Rendition [0..1]</iirds:description>
	</rdf:Property>
	<rdf:Property rdf:about="http://iirds.tekom.de/iirds#has-start-selector">
		<rdfs:label xml:lang="de">hat Startselektor</rdfs:label>
		<rdfs:label xml:lang="en">has start selector</rdfs:label>
		<rdfs:subPropertyOf rdf:resource="http://iirds.tekom.de/iirds#has-selector"/>
		<rdfs:domain rdf:resource="http://iirds.tekom.de/iirds#RangeSelector"/>
		<rdfs:range rdf:resource="http://iirds.tekom.de/iirds#FragmentSelector"/>
		<iirds:description xml:lang="en">A range selector must reference one start and one end selector.</iirds:description>
		<rdfs:comment xml:lang="en">range selector's property that references the start of its  range</rdfs:comment>
		<schema:domainIncludes rdf:resource="http://iirds.tekom.de/iirds#RangeSelector"/>
		<schema:rangeIncludes rdf:resource="http://iirds.tekom.de/iirds#FragmentSelector"/>
		<iirds:description xml:lang="en">Cardinality: http://iirds.tekom.de/iirds#RangeSelector [1]</iirds:description>
	</rdf:Property>
	<rdf:Property rdf:about="http://iirds.tekom.de/iirds#has-subject">
		<rdfs:label xml:lang="de">hat Thema</rdfs:label>
		<rdfs:label xml:lang="en">has subject</rdfs:label>
		<rdfs:subPropertyOf rdf:resource="http://purl.org/dc/terms/subject"/>
		<rdfs:subPropertyOf rdf:resource="http://iirds.tekom.de/iirds#has-information-type"/>
		<rdfs:domain rdf:resource="http://iirds.tekom.de/iirds#InformationUnit"/>
		<rdfs:range rdf:resource="http://iirds.tekom.de/iirds#InformationSubject"/>
		<iirds:description xml:lang="en"/>
		<rdfs:comment xml:lang="en">information unit's property that references its subject</rdfs:comment>
		<schema:domainIncludes rdf:resource="http://iirds.tekom.de/iirds#InformationUnit"/>
		<schema:rangeIncludes rdf:resource="http://iirds.tekom.de/iirds#InformationSubject"/>
		<iirds:description xml:lang="en">Cardinality: http://iirds.tekom.de/iirds#InformationUnit [0..*]</iirds:description>
	</rdf:Property>
	<rdf:Property rdf:about="http://iirds.tekom.de/iirds#has-topic-type">
		<rdfs:label xml:lang="de">hat Topictyp</rdfs:label>
		<rdfs:label xml:lang="en">has topic type</rdfs:label>
		<rdfs:subPropertyOf rdf:resource="http://iirds.tekom.de/iirds#has-information-type"/>
		<rdfs:domain rdf:resource="http://iirds.tekom.de/iirds#InformationUnit"/>
		<rdfs:range rdf:resource="http://iirds.tekom.de/iirds#TopicType"/>
		<iirds:description xml:lang="en">Defines the information type of a topic, e.g. task or learning.</iirds:description>
		<rdfs:comment xml:lang="en">information unit's property that references its topic type</rdfs:comment>
		<schema:domainIncludes rdf:resource="http://iirds.tekom.de/iirds#InformationUnit"/>
		<schema:rangeIncludes rdf:resource="http://iirds.tekom.de/iirds#TopicType"/>
		<iirds:description xml:lang="en">Cardinality: http://iirds.tekom.de/iirds#InformationUnit [0..*]</iirds:description>
	</rdf:Property>
	<rdf:Property rdf:about="http://iirds.tekom.de/iirds#iirdsRelationConcept">
		<rdfs:label xml:lang="de">iirdsRelationConcept</rdfs:label>
		<rdfs:label xml:lang="en">iirdsRelationConcept</rdfs:label>
		<rdfs:domain rdf:resource="http://iirds.tekom.de/iirds#iirdsDomainEntity"/>
		<rdfs:range rdf:resource="http://iirds.tekom.de/iirds#iirdsDomainEntity"/>
		<iirds:description xml:lang="en">Not indented to be used directly.</iirds:description>
		<rdfs:comment xml:lang="en">iiRDS resource's property that references an iiRDS resource</rdfs:comment>
		<schema:domainIncludes rdf:resource="http://iirds.tekom.de/iirds#iirdsDomainEntity"/>
		<schema:rangeIncludes rdf:resource="http://iirds.tekom.de/iirds#iirdsDomainEntity"/>
		<iirds:description xml:lang="en">Cardinality: http://iirds.tekom.de/iirds#iirdsDomainEntity [0..*]</iirds:description>
	</rdf:Property>
	<rdf:Property rdf:about="http://iirds.tekom.de/iirds#is-part-of-package">
		<rdfs:label xml:lang="de">ist Teil von Paket</rdfs:label>
		<rdfs:label xml:lang="en">is part of package</rdfs:label>
		<rdfs:subPropertyOf rdf:resource="http://iirds.tekom.de/iirds#iirdsRelationConcept"/>
		<rdfs:domain rdf:resource="http://iirds.tekom.de/iirds#InformationUnit"/>
		<rdfs:range rdf:resource="http://iirds.tekom.de/iirds#Package"/>
		<iirds:description xml:lang="en"/>
		<rdfs:comment xml:lang="en">information unit's property that references the package to which it belongs</rdfs:comment>
		<schema:domainIncludes rdf:resource="http://iirds.tekom.de/iirds#InformationUnit"/>
		<schema:rangeIncludes rdf:resource="http://iirds.tekom.de/iirds#Package"/>
		<iirds:description xml:lang="en">Cardinality: http://iirds.tekom.de/iirds#InformationUnit [0..*]</iirds:description>
	</rdf:Property>
	<rdf:Property rdf:about="http://iirds.tekom.de/iirds#is-replacement-of">
		<rdfs:label xml:lang="de">ersetzt</rdfs:label>
		<rdfs:label xml:lang="en">replaces</rdfs:label>
		<rdfs:subPropertyOf rdf:resource="http://purl.org/dc/terms/replaces"/>
		<rdfs:subPropertyOf rdf:resource="http://iirds.tekom.de/iirds#iirdsRelationConcept"/>
		<rdfs:domain rdf:resource="http://iirds.tekom.de/iirds#InformationUnit"/>
		<rdfs:range rdf:resource="http://iirds.tekom.de/iirds#InformationUnit"/>
		<iirds:description xml:lang="en"/>
		<rdfs:comment xml:lang="en">information unit's property that references the information unit to be replaced</rdfs:comment>
		<schema:domainIncludes rdf:resource="http://iirds.tekom.de/iirds#InformationUnit"/>
		<schema:rangeIncludes rdf:resource="http://iirds.tekom.de/iirds#InformationUnit"/>
		<iirds:description xml:lang="en">Cardinality: http://iirds.tekom.de/iirds#InformationUnit [0..1]</iirds:description>
	</rdf:Property>
	<rdf:Property rdf:about="http://iirds.tekom.de/iirds#is-version-of">
		<rdfs:label xml:lang="de">ist Version von</rdfs:label>
		<rdfs:label xml:lang="en">is version of</rdfs:label>
		<rdfs:subPropertyOf rdf:resource="http://iirds.tekom.de/iirds#iirdsRelationConcept"/>
		<rdfs:subPropertyOf rdf:resource="http://purl.org/dc/terms/isVersionOf"/>
		<rdfs:domain rdf:resource="http://iirds.tekom.de/iirds#InformationUnit"/>
		<rdfs:range rdf:resource="http://iirds.tekom.de/iirds#InformationObject"/>
		<iirds:description xml:lang="en">Specifies that the information unit is a version or language variant of the information object.</iirds:description>
		<rdfs:comment xml:lang="en">information unit's property that references its information object</rdfs:comment>
		<schema:domainIncludes rdf:resource="http://iirds.tekom.de/iirds#InformationUnit"/>
		<schema:rangeIncludes rdf:resource="http://iirds.tekom.de/iirds#InformationObject"/>
		<iirds:description xml:lang="en">Cardinality: http://iirds.tekom.de/iirds#InformationUnit [0..1]</iirds:description>
	</rdf:Property>
	<rdf:Property rdf:about="http://iirds.tekom.de/iirds#purpose">
		<rdfs:label xml:lang="de">Zweck</rdfs:label>
		<rdfs:label xml:lang="en">purpose</rdfs:label>
		<rdfs:subPropertyOf rdf:resource="http://iirds.tekom.de/iirds#iirdsAttribute"/>
		<rdfs:domain rdf:resource="http://iirds.tekom.de/iirds#ContentLifeCycleStatus"/>
		<rdfs:range rdf:resource="http://www.w3.org/2000/01/rdf-schema#Literal"/>
		<iirds:description xml:lang="en"/>
		<rdfs:comment xml:lang="en">reason for an information unit's lifecycle status</rdfs:comment>
		<schema:domainIncludes rdf:resource="http://iirds.tekom.de/iirds#ContentLifeCycleStatus"/>
		<schema:rangeIncludes rdf:resource="http://www.w3.org/2000/01/rdf-schema#Literal"/>
		<iirds:description xml:lang="en">Cardinality: http://iirds.tekom.de/iirds#ContentLifeCycleStatus [0..1]</iirds:description>
	</rdf:Property>
	<rdf:Property rdf:about="http://iirds.tekom.de/iirds#relates-to-action">
		<rdfs:label xml:lang="de">bezieht sich auf Handlung</rdfs:label>
		<rdfs:label xml:lang="en">relates to action</rdfs:label>
		<rdfs:subPropertyOf rdf:resource="http://iirds.tekom.de/iirds#relates-to-functional-metadata"/>
		<rdfs:domain rdf:resource="http://iirds.tekom.de/iirds#InformationUnit"/>
		<rdfs:range rdf:resource="http://iirds.tekom.de/iirds#Action"/>
		<iirds:description xml:lang="en">Not intended to be used directly. Use the subclasses instead.</iirds:description>
		<rdfs:comment xml:lang="en">information unit's property that references an action</rdfs:comment>
		<schema:domainIncludes rdf:resource="http://iirds.tekom.de/iirds#InformationUnit"/>
		<schema:rangeIncludes rdf:resource="http://iirds.tekom.de/iirds#Action"/>
		<iirds:description xml:lang="en">Cardinality: http://iirds.tekom.de/iirds#InformationUnit [0..*]</iirds:description>
	</rdf:Property>
	<rdf:Property rdf:about="http://iirds.tekom.de/iirds#relates-to-administrative-metadata">
		<rdfs:label xml:lang="de">bezieht sich auf administrative Metadaten</rdfs:label>
		<rdfs:label xml:lang="en">relates to administrative metadata</rdfs:label>
		<rdfs:subPropertyOf rdf:resource="http://iirds.tekom.de/iirds#iirdsRelationConcept"/>
		<rdfs:domain rdf:resource="http://iirds.tekom.de/iirds#iirdsDomainEntity"/>
		<rdfs:range rdf:resource="http://iirds.tekom.de/iirds#AdministrativeMetadata"/>
		<iirds:description xml:lang="en">Not intended to be used directly. Use the subclasses instead.</iirds:description>
		<rdfs:comment xml:lang="en">iiRDS resource's property that references administrative metadata </rdfs:comment>
		<schema:domainIncludes rdf:resource="http://iirds.tekom.de/iirds#iirdsDomainEntity"/>
		<schema:rangeIncludes rdf:resource="http://iirds.tekom.de/iirds#AdministrativeMetadata"/>
		<iirds:description xml:lang="en">Cardinality: http://iirds.tekom.de/iirds#iirdsDomainEntity [0..*]</iirds:description>
	</rdf:Property>
	<rdf:Property rdf:about="http://iirds.tekom.de/iirds#relates-to-component">
		<rdfs:label xml:lang="de">bezieht sich auf Komponente</rdfs:label>
		<rdfs:label xml:lang="en">relates to component</rdfs:label>
		<rdfs:subPropertyOf rdf:resource="http://iirds.tekom.de/iirds#relates-to-product-metadata"/>
		<rdfs:domain rdf:resource="http://iirds.tekom.de/iirds#InformationUnit"/>
		<rdfs:range rdf:resource="http://iirds.tekom.de/iirds#Component"/>
		<iirds:description xml:lang="en">That means that the content of the information unit relates to a specific component of the documented product or component.</iirds:description>
		<rdfs:comment xml:lang="en">information unit's property that references a component</rdfs:comment>
		<schema:domainIncludes rdf:resource="http://iirds.tekom.de/iirds#InformationUnit"/>
		<schema:rangeIncludes rdf:resource="http://iirds.tekom.de/iirds#Component"/>
		<iirds:description xml:lang="en">Cardinality: http://iirds.tekom.de/iirds#InformationUnit [0..*]</iirds:description>
	</rdf:Property>
	<rdf:Property rdf:about="http://iirds.tekom.de/iirds#relates-to-event">
		<rdfs:label xml:lang="de">bezieht sich auf Ereignis</rdfs:label>
		<rdfs:label xml:lang="en">relates to event</rdfs:label>
		<rdfs:subPropertyOf rdf:resource="http://iirds.tekom.de/iirds#relates-to-functional-metadata"/>
		<rdfs:domain rdf:resource="http://iirds.tekom.de/iirds#InformationUnit"/>
		<rdfs:range rdf:resource="http://iirds.tekom.de/iirds#Event"/>
		<iirds:description xml:lang="en">That means that the content of the information unit refers to a specific event that occured in the product/system, e.g. an error.</iirds:description>
		<rdfs:comment xml:lang="en">information unit's property that references an event</rdfs:comment>
		<schema:domainIncludes rdf:resource="http://iirds.tekom.de/iirds#InformationUnit"/>
		<schema:rangeIncludes rdf:resource="http://iirds.tekom.de/iirds#Event"/>
		<iirds:description xml:lang="en">Cardinality: http://iirds.tekom.de/iirds#InformationUnit [0..*]</iirds:description>
	</rdf:Property>
	<rdf:Property rdf:about="http://iirds.tekom.de/iirds#relates-to-functional-metadata">
		<rdfs:label xml:lang="de">bezieht sich auf funktionale Metadaten</rdfs:label>
		<rdfs:label xml:lang="en">relates to functional metadata</rdfs:label>
		<rdfs:subPropertyOf rdf:resource="http://iirds.tekom.de/iirds#iirdsRelationConcept"/>
		<rdfs:domain rdf:resource="http://iirds.tekom.de/iirds#InformationUnit"/>
		<rdfs:range rdf:resource="http://iirds.tekom.de/iirds#FunctionalMetadata"/>
		<iirds:description xml:lang="en">No intended to be used directly. Use the subclasses instead.</iirds:description>
		<rdfs:comment xml:lang="en">information unit's property that references functional metadata</rdfs:comment>
		<schema:domainIncludes rdf:resource="http://iirds.tekom.de/iirds#InformationUnit"/>
		<schema:rangeIncludes rdf:resource="http://iirds.tekom.de/iirds#FunctionalMetadata"/>
		<iirds:description xml:lang="en">Cardinality: http://iirds.tekom.de/iirds#InformationUnit [0..*]</iirds:description>
	</rdf:Property>
	<rdf:Property rdf:about="http://iirds.tekom.de/iirds#relates-to-information-unit">
		<rdfs:label xml:lang="de">bezieht sich auf Informationseinheit</rdfs:label>
		<rdfs:label xml:lang="en">relates to information unit</rdfs:label>
		<rdfs:subPropertyOf rdf:resource="http://iirds.tekom.de/iirds#iirdsRelationConcept"/>
		<rdfs:domain rdf:resource="http://iirds.tekom.de/iirds#DirectoryNode"/>
		<rdfs:range rdf:resource="http://iirds.tekom.de/iirds#InformationUnit"/>
		<iirds:description xml:lang="en">The related information unit is part of the directory.</iirds:description>
		<rdfs:comment xml:lang="en">directory node's property that references the corresponding information unit</rdfs:comment>
		<schema:domainIncludes rdf:resource="http://iirds.tekom.de/iirds#DirectoryNode"/>
		<schema:rangeIncludes rdf:resource="http://iirds.tekom.de/iirds#InformationUnit"/>
		<iirds:description xml:lang="en">Cardinality: http://iirds.tekom.de/iirds#DirectoryNode [0..1]</iirds:description>
	</rdf:Property>
	<rdf:Property rdf:about="http://iirds.tekom.de/iirds#relates-to-party">
		<rdfs:label xml:lang="de">hat Beziehung zu Akteur</rdfs:label>
		<rdfs:label xml:lang="en">relates to party</rdfs:label>
		<rdfs:subPropertyOf rdf:resource="http://iirds.tekom.de/iirds#relates-to-administrative-metadata"/>
		<rdfs:range rdf:resource="http://iirds.tekom.de/iirds#Party"/>
		<iirds:description xml:lang="en"/>
		<rdfs:comment xml:lang="en">iiRDS resource's property that references a party</rdfs:comment>
		<schema:domainIncludes rdf:resource="http://iirds.tekom.de/iirds#Component"/>
		<schema:domainIncludes rdf:resource="http://iirds.tekom.de/iirds#IdentityDomain"/>
		<schema:domainIncludes rdf:resource="http://iirds.tekom.de/iirds#ClassificationDomain"/>
		<schema:domainIncludes rdf:resource="http://iirds.tekom.de/iirds#InformationUnit"/>
		<schema:domainIncludes rdf:resource="http://iirds.tekom.de/iirds#ContentLifeCycleStatus"/>
		<schema:domainIncludes rdf:resource="http://iirds.tekom.de/iirds#ProductVariant"/>
		<schema:rangeIncludes rdf:resource="http://iirds.tekom.de/iirds#Party"/>
		<iirds:description xml:lang="en">Cardinality: http://iirds.tekom.de/iirds#Component [0..1]</iirds:description>
		<iirds:description xml:lang="en">Cardinality: http://iirds.tekom.de/iirds#ContentLifeCycleStatus [0..1]</iirds:description>
		<iirds:description xml:lang="en">Cardinality: http://iirds.tekom.de/iirds#InformationUnit [0..*]</iirds:description>
		<iirds:description xml:lang="en">Cardinality: http://iirds.tekom.de/iirds#IdentityDomain [0..1]</iirds:description>
		<iirds:description xml:lang="en">Cardinality: http://iirds.tekom.de/iirds#ClassificationDomain [0..1]</iirds:description>
		<iirds:description xml:lang="en">Cardinality: http://iirds.tekom.de/iirds#ProductVariant [0..1]</iirds:description>
	</rdf:Property>
	<rdf:Property rdf:about="http://iirds.tekom.de/iirds#relates-to-product-feature">
		<rdfs:label xml:lang="de">bezieht sich auf Produkteigenschaft</rdfs:label>
		<rdfs:label xml:lang="en">relates to product feature</rdfs:label>
		<rdfs:subPropertyOf rdf:resource="http://iirds.tekom.de/iirds#relates-to-product-metadata"/>
		<rdfs:domain rdf:resource="http://iirds.tekom.de/iirds#InformationUnit"/>
		<rdfs:range rdf:resource="http://iirds.tekom.de/iirds#ProductFeature"/>
		<iirds:description xml:lang="en">That means that the content of the information unit refers to or describes a specific product feature.</iirds:description>
		<rdfs:comment xml:lang="en">information unit's property that references a product feature</rdfs:comment>
		<schema:domainIncludes rdf:resource="http://iirds.tekom.de/iirds#InformationUnit"/>
		<schema:rangeIncludes rdf:resource="http://iirds.tekom.de/iirds#ProductFeature"/>
		<iirds:description xml:lang="en">Cardinality: http://iirds.tekom.de/iirds#InformationUnit [0..*]</iirds:description>
	</rdf:Property>
	<rdf:Property rdf:about="http://iirds.tekom.de/iirds#relates-to-product-lifecycle-phase">
		<rdfs:label xml:lang="de">bezieht sich auf Produktlebenszyklusphase</rdfs:label>
		<rdfs:label xml:lang="en">relates to phase of the product lifecycle</rdfs:label>
		<rdfs:subPropertyOf rdf:resource="http://iirds.tekom.de/iirds#relates-to-product-metadata"/>
		<rdfs:domain rdf:resource="http://iirds.tekom.de/iirds#InformationUnit"/>
		<rdfs:range rdf:resource="http://iirds.tekom.de/iirds#ProductLifeCyclePhase"/>
		<iirds:description xml:lang="en">That means that the content of the information unit describes activities or knowledge related to a specific lifecycle phase. Examples are operation and maintenance.</iirds:description>
		<rdfs:comment xml:lang="en">information unit's property that references a product lifecycle phase</rdfs:comment>
		<schema:domainIncludes rdf:resource="http://iirds.tekom.de/iirds#InformationUnit"/>
		<schema:rangeIncludes rdf:resource="http://iirds.tekom.de/iirds#ProductLifeCyclePhase"/>
		<iirds:description xml:lang="en">Cardinality: http://iirds.tekom.de/iirds#InformationUnit [0..*]</iirds:description>
	</rdf:Property>
	<rdf:Property rdf:about="http://iirds.tekom.de/iirds#relates-to-product-metadata">
		<rdfs:label xml:lang="de">bezieht sich auf Produktmetadaten</rdfs:label>
		<rdfs:label xml:lang="en">relates to product metadata</rdfs:label>
		<rdfs:subPropertyOf rdf:resource="http://iirds.tekom.de/iirds#iirdsRelationConcept"/>
		<rdfs:domain rdf:resource="http://iirds.tekom.de/iirds#InformationUnit"/>
		<rdfs:range rdf:resource="http://iirds.tekom.de/iirds#ProductMetadata"/>
		<iirds:description xml:lang="en"/>
		<rdfs:comment xml:lang="en">information unit's property that references product metadata</rdfs:comment>
		<schema:domainIncludes rdf:resource="http://iirds.tekom.de/iirds#InformationUnit"/>
		<schema:rangeIncludes rdf:resource="http://iirds.tekom.de/iirds#ProductMetadata"/>
		<iirds:description xml:lang="en">Cardinality: http://iirds.tekom.de/iirds#InformationUnit [0..*]</iirds:description>
	</rdf:Property>
	<rdf:Property rdf:about="http://iirds.tekom.de/iirds#relates-to-product-variant">
		<rdfs:label xml:lang="de">bezieht sich auf Produktvariante</rdfs:label>
		<rdfs:label xml:lang="en">relates to product variant</rdfs:label>
		<rdfs:subPropertyOf rdf:resource="http://iirds.tekom.de/iirds#relates-to-product-metadata"/>
		<rdfs:domain rdf:resource="http://iirds.tekom.de/iirds#InformationUnit"/>
		<rdfs:range rdf:resource="http://iirds.tekom.de/iirds#ProductVariant"/>
		<iirds:description xml:lang="en">That means that the content of the information unit refers to or describes a specific variant of the product.</iirds:description>
		<rdfs:comment xml:lang="en">information unit's property that references a product variant</rdfs:comment>
		<schema:domainIncludes rdf:resource="http://iirds.tekom.de/iirds#InformationUnit"/>
		<schema:rangeIncludes rdf:resource="http://iirds.tekom.de/iirds#ProductVariant"/>
		<iirds:description xml:lang="en">Cardinality: http://iirds.tekom.de/iirds#InformationUnit [0..*]</iirds:description>
	</rdf:Property>
	<rdf:Property rdf:about="http://iirds.tekom.de/iirds#relates-to-qualification">
		<rdfs:label xml:lang="de">bezieht sich auf Qualifikation</rdfs:label>
		<rdfs:label xml:lang="en">relates to qualification</rdfs:label>
		<rdfs:subPropertyOf rdf:resource="http://iirds.tekom.de/iirds#relates-to-functional-metadata"/>
		<rdfs:domain rdf:resource="http://iirds.tekom.de/iirds#InformationUnit"/>
		<rdfs:range rdf:resource="http://iirds.tekom.de/iirds#Qualification"/>
		<iirds:description xml:lang="en"/>
		<rdfs:comment xml:lang="en">information unit's property that references a qualification </rdfs:comment>
		<schema:domainIncludes rdf:resource="http://iirds.tekom.de/iirds#InformationUnit"/>
		<schema:rangeIncludes rdf:resource="http://iirds.tekom.de/iirds#Qualification"/>
		<iirds:description xml:lang="en">Cardinality: http://iirds.tekom.de/iirds#InformationUnit [0..*]</iirds:description>
	</rdf:Property>
	<rdf:Property rdf:about="http://iirds.tekom.de/iirds#relates-to-supply">
		<rdfs:label xml:lang="de">bezieht sich auf Hilfsmittel</rdfs:label>
		<rdfs:label xml:lang="en">relates to supply</rdfs:label>
		<rdfs:subPropertyOf rdf:resource="http://iirds.tekom.de/iirds#relates-to-functional-metadata"/>
		<rdfs:domain rdf:resource="http://iirds.tekom.de/iirds#InformationUnit"/>
		<rdfs:range rdf:resource="http://iirds.tekom.de/iirds#Supply"/>
		<iirds:description xml:lang="en"/>
		<rdfs:comment xml:lang="en">information unit's property that references a supply</rdfs:comment>
		<schema:domainIncludes rdf:resource="http://iirds.tekom.de/iirds#InformationUnit"/>
		<schema:rangeIncludes rdf:resource="http://iirds.tekom.de/iirds#Supply"/>
		<iirds:description xml:lang="en">Cardinality: http://iirds.tekom.de/iirds#InformationUnit [0..*]</iirds:description>
	</rdf:Property>
	<rdf:Property rdf:about="http://iirds.tekom.de/iirds#relates-to-vcard">
		<rdfs:label xml:lang="de">bezieht sich auf vCard</rdfs:label>
		<rdfs:label xml:lang="en">relates to vCard</rdfs:label>
		<rdfs:subPropertyOf rdf:resource="http://iirds.tekom.de/iirds#iirdsRelationConcept"/>
		<rdfs:domain rdf:resource="http://iirds.tekom.de/iirds#Party"/>
		<rdfs:range rdf:resource="http://www.w3.org/2006/vcard/ns#Kind"/>
		<iirds:description xml:lang="en"/>
		<rdfs:comment xml:lang="en">party's property that references an organization or person</rdfs:comment>
		<schema:domainIncludes rdf:resource="http://iirds.tekom.de/iirds#Party"/>
		<schema:rangeIncludes rdf:resource="http://www.w3.org/2006/vcard/ns#Kind"/>
		<iirds:description xml:lang="en">Cardinality: http://iirds.tekom.de/iirds#Party [0..1]</iirds:description>
	</rdf:Property>
	<iirds:Action rdf:about="http://iirds.tekom.de/iirds#GenericAction">
		<rdfs:label xml:lang="de">Handlung</rdfs:label>
		<rdfs:label xml:lang="en">action</rdfs:label>
		<iirds:description xml:lang="en"/>
		<rdfs:comment xml:lang="en">atomic manipulation of an object by a participant</rdfs:comment>
	</iirds:Action>
	<iirds:DesignAndRealization rdf:about="http://iirds.tekom.de/iirds#Acquisition">
		<rdfs:label xml:lang="de">Beschaffung</rdfs:label>
		<rdfs:label xml:lang="en">acquisition</rdfs:label>
		<iirds:description xml:lang="en"/>
		<rdfs:comment xml:lang="en">product life cycle phase of obtaining systems, products, or services as part of design and realization</rdfs:comment>
	</iirds:DesignAndRealization>
	<iirds:DocumentType rdf:about="http://iirds.tekom.de/iirds#AdministratorGuide">
		<rdfs:label xml:lang="de">Administrationsanleitung</rdfs:label>
		<rdfs:label xml:lang="en">administrator guide</rdfs:label>
		<iirds:description xml:lang="en"/>
		<rdfs:comment xml:lang="en">document type that refers to information on the management of a technical system</rdfs:comment>
	</iirds:DocumentType>
	<iirds:Conformity rdf:about="http://iirds.tekom.de/iirds#ApplicableStandards">
		<rdfs:label xml:lang="de">Geltende Norm und Richtlinie</rdfs:label>
		<rdfs:label xml:lang="en">applicable standard</rdfs:label>
		<iirds:description xml:lang="en">Examples: machinery directive, ATEX directive</iirds:description>
		<rdfs:comment xml:lang="en">information subject covering rules, guidelines, or definitions of product characteristics that need to comply with normative or legislative requirements</rdfs:comment>
	</iirds:Conformity>
	<iirds:DocumentType rdf:about="http://iirds.tekom.de/iirds#AssemblyInstructions">
		<rdfs:label xml:lang="de">Montageanleitung</rdfs:label>
		<rdfs:label xml:lang="en">assembly instructions</rdfs:label>
		<iirds:description xml:lang="en"/>
		<rdfs:comment xml:lang="en">document type that refers to information on how parts are put together to complete a specific product so that it fulfils its intended use</rdfs:comment>
	</iirds:DocumentType>
	<iirds:DocumentType rdf:about="http://iirds.tekom.de/iirds#CEDeclarationOfConformity">
		<rdfs:label xml:lang="de">CE-Konformitätserklärung</rdfs:label>
		<rdfs:label xml:lang="en">cE declaration of conformity</rdfs:label>
		<iirds:description xml:lang="en"/>
		<rdfs:comment xml:lang="en">document type that refers to a confirmation that a product complies with the applicable CE marking directives or regulations</rdfs:comment>
	</iirds:DocumentType>
	<iirds:PuttingToUse rdf:about="http://iirds.tekom.de/iirds#Configuration">
		<rdfs:label xml:lang="de">Einrichtung</rdfs:label>
		<rdfs:label xml:lang="en">configuration</rdfs:label>
		<iirds:description xml:lang="en"/>
		<rdfs:comment xml:lang="en">product life cycle phase of adapting settings to achieve the desired functionality of a product</rdfs:comment>
	</iirds:PuttingToUse>
	<iirds:Formality rdf:about="http://iirds.tekom.de/iirds#ContactInformation">
		<rdfs:label xml:lang="de">Kontaktdaten</rdfs:label>
		<rdfs:label xml:lang="en">contact information</rdfs:label>
		<iirds:description xml:lang="en">Contact information such as addresses, phone numbers, URLs.</iirds:description>
		<rdfs:comment xml:lang="en">information subject that covers information on how to contact a party</rdfs:comment>
	</iirds:Formality>
	<iirds:Conformity rdf:about="http://iirds.tekom.de/iirds#DeclarationOfConformity">
		<rdfs:label xml:lang="de">Konformitätserklärung</rdfs:label>
		<rdfs:label xml:lang="en">declaration of conformity</rdfs:label>
		<iirds:description xml:lang="en">The Declaration of Conformity states that the product complies with the essential requirements of the relevant standards. </iirds:description>
		<rdfs:comment xml:lang="en">information subject covering an assurance that the product complies  with the EU Declaration of Conformity for CE marking</rdfs:comment>
	</iirds:Conformity>
	<iirds:Use rdf:about="http://iirds.tekom.de/iirds#Decommissioning">
		<rdfs:label xml:lang="de">Außerbetriebnahme</rdfs:label>
		<rdfs:label xml:lang="en">decommissioning</rdfs:label>
		<iirds:description xml:lang="en"/>
		<rdfs:comment xml:lang="en">product life cycle phase of shutting down a system at the end of its usage period</rdfs:comment>
	</iirds:Use>
	<iirds:DesignAndRealization rdf:about="http://iirds.tekom.de/iirds#Design">
		<rdfs:label xml:lang="de">Design</rdfs:label>
		<rdfs:label xml:lang="en">design</rdfs:label>
		<iirds:description xml:lang="en"/>
		<rdfs:comment xml:lang="en">product life cycle phase of designing systems, products, or services</rdfs:comment>
	</iirds:DesignAndRealization>
	<iirds:DesignAndRealization rdf:about="http://iirds.tekom.de/iirds#Development">
		<rdfs:label xml:lang="de">Entwicklung</rdfs:label>
		<rdfs:label xml:lang="en">development</rdfs:label>
		<iirds:description xml:lang="en"/>
		<rdfs:comment xml:lang="en">product life cycle phase of transfoming from design into a production-ready functional system, product or service</rdfs:comment>
	</iirds:DesignAndRealization>
	<iirds:Use rdf:about="http://iirds.tekom.de/iirds#Diagnostics">
		<rdfs:label xml:lang="de">Fehlerdiagnose</rdfs:label>
		<rdfs:label xml:lang="en">diagnostics</rdfs:label>
		<iirds:description xml:lang="en"/>
		<rdfs:comment xml:lang="en">product life cycle phase of identifying a fault and its cause whitin the use phase</rdfs:comment>
	</iirds:Use>
	<iirds:AfterUse rdf:about="http://iirds.tekom.de/iirds#Disposal">
		<rdfs:label xml:lang="de">Entsorgung</rdfs:label>
		<rdfs:label xml:lang="en">disposal</rdfs:label>
		<iirds:description xml:lang="en"/>
		<rdfs:comment xml:lang="en">product life cycle phase spanning the process of elimination of a product or component</rdfs:comment>
	</iirds:AfterUse>
	<iirds:Use rdf:about="http://iirds.tekom.de/iirds#EmergencyOperation">
		<rdfs:label xml:lang="de">Notbetrieb</rdfs:label>
		<rdfs:label xml:lang="en">emergency operation</rdfs:label>
		<iirds:description xml:lang="en"/>
		<rdfs:comment xml:lang="en">product life cycle of restricted operation of a system to protect it from damage</rdfs:comment>
	</iirds:Use>
	<iirds:Use rdf:about="http://iirds.tekom.de/iirds#Fault">
		<rdfs:label xml:lang="de">Störung</rdfs:label>
		<rdfs:label xml:lang="en">fault</rdfs:label>
		<iirds:description xml:lang="en"/>
		<rdfs:comment xml:lang="en">product life cycle that spans the interruption of the intended operation of a system due to malfunction</rdfs:comment>
	</iirds:Use>
	<iirds:Safety rdf:about="http://iirds.tekom.de/iirds#ForeseeableMisuse">
		<rdfs:label xml:lang="de">Vorhersehbarer Fehlgebrauch</rdfs:label>
		<rdfs:label xml:lang="en">foreseeable misuse</rdfs:label>
		<iirds:description xml:lang="en">Use of a product in a manner not intended by the producer or supplier but which may result from foreseeable human behavior. See EN 82079-1</iirds:description>
		<rdfs:comment xml:lang="en">information subject that covers the use of a product or system in a way not intended by the supplier, but which can result from readily predictable human behaviour</rdfs:comment>
	</iirds:Safety>
	<iirds:AfterUse rdf:about="http://iirds.tekom.de/iirds#GenericAfterUse">
		<rdfs:label xml:lang="de">Nutzungsende</rdfs:label>
		<rdfs:label xml:lang="en">after use</rdfs:label>
		<iirds:description xml:lang="en">The AfterUse class is a parent class for product lifecycle phases that occur after the active use of the product.</iirds:description>
		<rdfs:comment xml:lang="en">product life cycle phase following the active use of the product</rdfs:comment>
	</iirds:AfterUse>
	<iirds:Collection rdf:about="http://iirds.tekom.de/iirds#GenericCollection">
		<rdfs:label xml:lang="de">Zusammenstellung</rdfs:label>
		<rdfs:label xml:lang="en">collection</rdfs:label>
		<iirds:description xml:lang="en"/>
		<rdfs:comment xml:lang="en">information subject covering specific content in lists or overviews</rdfs:comment>
	</iirds:Collection>
	<iirds:Concept rdf:about="http://iirds.tekom.de/iirds#GenericConcept">
		<rdfs:label xml:lang="de">Beschreibung</rdfs:label>
		<rdfs:label xml:lang="en">concept</rdfs:label>
		<iirds:description xml:lang="en">Conceptual information helps users to map their existing knowledge to tasks and other essential information about a product or system.</iirds:description>
		<rdfs:comment xml:lang="en">topic type providing background information that helps users understand the structure or essential principles of a product, interface, or task</rdfs:comment>
	</iirds:Concept>
	<iirds:Conformity rdf:about="http://iirds.tekom.de/iirds#GenericConformity">
		<rdfs:label xml:lang="de">Konformität</rdfs:label>
		<rdfs:label xml:lang="en">conformity</rdfs:label>
		<iirds:description xml:lang="en">The Conformity class is a parent class for information subjects that describe content related to applicable standards or the conformity of the product.</iirds:description>
		<rdfs:comment xml:lang="en">information subject covering applicable law, standards, or the fulfilment of a product requirement</rdfs:comment>
	</iirds:Conformity>
	<iirds:DesignAndRealization rdf:about="http://iirds.tekom.de/iirds#GenericDesignAndRealization">
		<rdfs:label xml:lang="de">Produktentstehung</rdfs:label>
		<rdfs:label xml:lang="en">design and realization</rdfs:label>
		<iirds:description xml:lang="en">The DesignAndRealization class is a parent class for product lifecycle phases related to the design, construction, and realization of a product.</iirds:description>
		<rdfs:comment xml:lang="en">product life cycle phase from ideation through production</rdfs:comment>
	</iirds:DesignAndRealization>
	<iirds:DownTime rdf:about="http://iirds.tekom.de/iirds#GenericDownTime">
		<rdfs:label xml:lang="de">Stillstandszeit</rdfs:label>
		<rdfs:label xml:lang="en">down time</rdfs:label>
		<iirds:description xml:lang="en">The DownTime class is a parent class for time periods during which an equipment or machine is not functional or cannot work.</iirds:description>
		<rdfs:comment xml:lang="en">period of time during which an item is not in condition to perform its intended function</rdfs:comment>
		<iirds:duration rdf:datatype="http://www.w3.org/2001/XMLSchema#duration">PT0M</iirds:duration>
	</iirds:DownTime>
	<iirds:Event rdf:about="http://iirds.tekom.de/iirds#GenericEvent">
		<rdfs:label xml:lang="de">Ereignis</rdfs:label>
		<rdfs:label xml:lang="en">event</rdfs:label>
		<iirds:description xml:lang="en">The Event class describes events that happen in the technical system. Examples are errors, malfunctions, and warnings.</iirds:description>
		<rdfs:comment xml:lang="en">something noticeable that takes place at a given location and point in time</rdfs:comment>
	</iirds:Event>
	<iirds:ContentLifeCycleStatusValue rdf:about="http://iirds.tekom.de/iirds#Approved">
		<rdfs:label xml:lang="de">Freigegeben</rdfs:label>
		<rdfs:label xml:lang="en">approved</rdfs:label>
		<iirds:description xml:lang="en"/>
		<rdfs:comment xml:lang="en">content life cycle status value which indicates that the information of the resource is correct</rdfs:comment>
	</iirds:ContentLifeCycleStatusValue>
	<iirds:ContentLifeCycleStatusValue rdf:about="http://iirds.tekom.de/iirds#Deleted">
		<rdfs:label xml:lang="de">Gelöscht</rdfs:label>
		<rdfs:label xml:lang="en">deleted</rdfs:label>
		<iirds:description xml:lang="en"/>
		<rdfs:comment xml:lang="en">content life cycle status value which indicates that the information of the resource has been revoked</rdfs:comment>
	</iirds:ContentLifeCycleStatusValue>
	<iirds:ContentLifeCycleStatusValue rdf:about="http://iirds.tekom.de/iirds#InPreparation">
		<rdfs:label xml:lang="de">In Arbeit</rdfs:label>
		<rdfs:label xml:lang="en">in preparation</rdfs:label>
		<iirds:description xml:lang="en"/>
		<rdfs:comment xml:lang="en">content life cycle status value which indicates that the information of the resource is still being edited</rdfs:comment>
	</iirds:ContentLifeCycleStatusValue>
	<iirds:ContentLifeCycleStatusValue rdf:about="http://iirds.tekom.de/iirds#InReview">
		<rdfs:label xml:lang="de">In Review</rdfs:label>
		<rdfs:label xml:lang="en">in review</rdfs:label>
		<iirds:description xml:lang="en"/>
		<rdfs:comment xml:lang="en">content life cycle status value which indicates that the information of the resource is being checked for correctness</rdfs:comment>
	</iirds:ContentLifeCycleStatusValue>
	<iirds:ContentLifeCycleStatusValue rdf:about="http://iirds.tekom.de/iirds#Released">
		<rdfs:label xml:lang="de">Veröffentlicht</rdfs:label>
		<rdfs:label xml:lang="en">released</rdfs:label>
		<iirds:description xml:lang="en"/>
		<rdfs:comment xml:lang="en">content life cycle status value which indicates that the associated information of the resource has been approved and is ready for publishing</rdfs:comment>
	</iirds:ContentLifeCycleStatusValue>
	<iirds:ContentLifeCycleStatusValue rdf:about="http://iirds.tekom.de/iirds#Reviewed">
		<rdfs:label xml:lang="de">Review durchgeführt</rdfs:label>
		<rdfs:label xml:lang="en">reviewed</rdfs:label>
		<iirds:description xml:lang="en"/>
		<rdfs:comment xml:lang="en">content life cycle status value which indicates that the information of the resource has been checked</rdfs:comment>
	</iirds:ContentLifeCycleStatusValue>
	<iirds:ContentLifeCycleStatusValue rdf:about="http://iirds.tekom.de/iirds#Withdrawn">
		<rdfs:label xml:lang="de">Widerrufen</rdfs:label>
		<rdfs:label xml:lang="en">withdrawn</rdfs:label>
		<iirds:description xml:lang="en"/>
		<rdfs:comment xml:lang="en">content life cycle status value which indicates that an already released information of the resource is not valid anymore</rdfs:comment>
	</iirds:ContentLifeCycleStatusValue>
	<iirds:Form rdf:about="http://iirds.tekom.de/iirds#GenericForm">
		<rdfs:label xml:lang="de">Formular</rdfs:label>
		<rdfs:label xml:lang="en">form</rdfs:label>
		<iirds:description xml:lang="en">The Form class describes topics that contain information in pre-defined form fields. Examples of forms are service reports, field reports, and user feedback.</iirds:description>
		<rdfs:comment xml:lang="en">topic type providing information in pre-defined fields</rdfs:comment>
	</iirds:Form>
	<iirds:Formality rdf:about="http://iirds.tekom.de/iirds#GenericFormality">
		<rdfs:label xml:lang="de">Formalie</rdfs:label>
		<rdfs:label xml:lang="en">formality</rdfs:label>
		<iirds:description xml:lang="en">The Formality class is the parent class for information subjects that describe content related to official or legal documents.</iirds:description>
		<rdfs:comment xml:lang="en">information subject that covers contractually relevant elements</rdfs:comment>
	</iirds:Formality>
	<iirds:Functionality rdf:about="http://iirds.tekom.de/iirds#GenericFunctionality">
		<rdfs:label xml:lang="de">Funktionalität</rdfs:label>
		<rdfs:label xml:lang="en">functionality</rdfs:label>
		<iirds:description xml:lang="en">The Functionality class is the parent class for information subjects that describe content related to specific functionalities of the product.</iirds:description>
		<rdfs:comment xml:lang="en">information subject that covers specific capabilities of the product</rdfs:comment>
	</iirds:Functionality>
	<iirds:Learning rdf:about="http://iirds.tekom.de/iirds#GenericLearning">
		<rdfs:label xml:lang="de">Lernen</rdfs:label>
		<rdfs:label xml:lang="en">learning</rdfs:label>
		<iirds:description xml:lang="en">Learning content may comprise learning plans, learning objectives, learning content details, summaries, and assessments.</iirds:description>
		<rdfs:comment xml:lang="en">type of topic that provides learning content</rdfs:comment>
	</iirds:Learning>
	<iirds:MaintenanceInterval rdf:about="http://iirds.tekom.de/iirds#GenericMaintenanceInterval">
		<rdfs:label xml:lang="de">Wartungsintervall</rdfs:label>
		<rdfs:label xml:lang="en">maintenance interval</rdfs:label>
		<iirds:description xml:lang="en">The MaintenanceInterval class describes time intervals and durations for the scheduled maintenance of a technical system or its parts.</iirds:description>
		<rdfs:comment xml:lang="en">period of time between scheduled maintenance operations</rdfs:comment>
		<iirds:duration rdf:datatype="http://www.w3.org/2001/XMLSchema#duration">PT0M</iirds:duration>
		<iirds:frequency>unknown</iirds:frequency>
	</iirds:MaintenanceInterval>
	<iirds:PartyRole rdf:about="http://iirds.tekom.de/iirds#Author">
		<rdfs:label xml:lang="de">Autor</rdfs:label>
		<rdfs:label xml:lang="en">author</rdfs:label>
		<iirds:description xml:lang="en">An author is the individual or the organization from which the referenced iiRDS domain entity originates.</iirds:description>
		<rdfs:comment xml:lang="en">party role of the party that edited the referenced information unit </rdfs:comment>
	</iirds:PartyRole>
	<iirds:PartyRole rdf:about="http://iirds.tekom.de/iirds#Creator">
		<rdfs:label xml:lang="de">Ersteller</rdfs:label>
		<rdfs:label xml:lang="en">creator</rdfs:label>
		<iirds:description xml:lang="en">A creator is the individual or the organization that created the referenced iiRDS domain entity.</iirds:description>
		<rdfs:comment xml:lang="en">party role of the party from which an information unit originated</rdfs:comment>
	</iirds:PartyRole>
	<iirds:PartyRole rdf:about="http://iirds.tekom.de/iirds#Contributor">
		<rdfs:label xml:lang="de">Beteiligter</rdfs:label>
		<rdfs:label xml:lang="en">contributor</rdfs:label>
		<iirds:description xml:lang="en">A contributor is an individual or an organization that participated in the generation/change of the referenced iiRDS domain entity.</iirds:description>
		<rdfs:comment xml:lang="en">party role of the party that provides input to the making of an information unit</rdfs:comment>
	</iirds:PartyRole>
	<iirds:PartyRole rdf:about="http://iirds.tekom.de/iirds#Customer">
		<rdfs:label xml:lang="de">Kunde</rdfs:label>
		<rdfs:label xml:lang="en">customer</rdfs:label>
		<iirds:description xml:lang="en">A customer is an individual or an organization that purchased or consumes the referenced iiRDS domain entity.</iirds:description>
		<rdfs:comment xml:lang="en">party role of the party that purchases or receives a product</rdfs:comment>
	</iirds:PartyRole>
	<iirds:PartyRole rdf:about="http://iirds.tekom.de/iirds#Inspector">
		<rdfs:label xml:lang="de">Prüfer</rdfs:label>
		<rdfs:label xml:lang="en">inspector</rdfs:label>
		<iirds:description xml:lang="en">An inspector is an individual or an organization that supervises or checks the referenced iiRDS domain entity and makes reports.</iirds:description>
		<rdfs:comment xml:lang="en">party role of the party that evaluates conformity with the requirements</rdfs:comment>
	</iirds:PartyRole>
	<iirds:PartyRole rdf:about="http://iirds.tekom.de/iirds#Manufacturer">
		<rdfs:label xml:lang="de">Hersteller</rdfs:label>
		<rdfs:label xml:lang="en">manufacturer</rdfs:label>
		<iirds:description xml:lang="en">The manufacturer is the individual or the organization that produces the referenced iiRDS domain entity.</iirds:description>
		<rdfs:comment xml:lang="en">party role of the party that designs or produces a product</rdfs:comment>
	</iirds:PartyRole>
	<iirds:PartyRole rdf:about="http://iirds.tekom.de/iirds#PerformedBy">
		<rdfs:label xml:lang="de">Durchgeführt von</rdfs:label>
		<rdfs:label xml:lang="en">performed by</rdfs:label>
		<iirds:description xml:lang="en">Describes the actor that is involved in changing the content lifecycle status.</iirds:description>
		<rdfs:comment xml:lang="en">party role of the party that changes the content life cycle status</rdfs:comment>
	</iirds:PartyRole>
	<iirds:PartyRole rdf:about="http://iirds.tekom.de/iirds#Supplier">
		<rdfs:label xml:lang="de">Zulieferer</rdfs:label>
		<rdfs:label xml:lang="en">supplier</rdfs:label>
		<iirds:description xml:lang="en">Describes the individual or the organization that provides the referenced iiRDS domain entity, e.g. a component.</iirds:description>
		<rdfs:comment xml:lang="en">party role of the party that provides products</rdfs:comment>
	</iirds:PartyRole>
	<iirds:PlanningTime rdf:about="http://iirds.tekom.de/iirds#GenericPlanningTime">
		<rdfs:label xml:lang="de">Planungszeit</rdfs:label>
		<rdfs:label xml:lang="en">planning time</rdfs:label>
		<iirds:description xml:lang="en">The PlanningTime class describes different types of planning times that may be referenced in technical documentation, for example time required for or resulting from specific working tasks.</iirds:description>
		<rdfs:comment xml:lang="en">period of time that is required for conducting a specific task</rdfs:comment>
		<iirds:duration rdf:datatype="http://www.w3.org/2001/XMLSchema#duration">PT0M</iirds:duration>
	</iirds:PlanningTime>
	<iirds:Process rdf:about="http://iirds.tekom.de/iirds#GenericProcess">
		<rdfs:label xml:lang="de">Prozess</rdfs:label>
		<rdfs:label xml:lang="en">process</rdfs:label>
		<iirds:description xml:lang="en">The Process class contains information subject for process-related information.</iirds:description>
		<rdfs:comment xml:lang="en">information subject that covers structured activities which are carried out to achieve a specific goal</rdfs:comment>
	</iirds:Process>
	<iirds:ProductFeature rdf:about="http://iirds.tekom.de/iirds#GenericProductFeature">
		<rdfs:label xml:lang="de">Produktmerkmal</rdfs:label>
		<rdfs:label xml:lang="en">product feature</rdfs:label>
		<iirds:description xml:lang="en">The ProductFeature class is a parent class for characteristics and functions of a product or component.</iirds:description>
		<rdfs:comment xml:lang="en">product characteristics</rdfs:comment>
	</iirds:ProductFeature>
	<iirds:ProductProperty rdf:about="http://iirds.tekom.de/iirds#GenericProductProperty">
		<rdfs:label xml:lang="de">Produkteigenschaft</rdfs:label>
		<rdfs:label xml:lang="en">product property</rdfs:label>
		<iirds:description xml:lang="en">The ProductProperty class describes a characteristic of a product or component.</iirds:description>
		<rdfs:comment xml:lang="en">invariable characteristic of a product whose value is fixed once the product is defined</rdfs:comment>
	</iirds:ProductProperty>
	<iirds:ProductFunction rdf:about="http://iirds.tekom.de/iirds#GenericProductFunction">
		<rdfs:label xml:lang="de">Produktfunktion</rdfs:label>
		<rdfs:label xml:lang="en">product function</rdfs:label>
		<iirds:description xml:lang="en">The ProductFunction class describes a function that a product or component provides or implements.</iirds:description>
		<rdfs:comment xml:lang="en">capability of a product or a component which is specific or required for the intended product task</rdfs:comment>
	</iirds:ProductFunction>
	<iirds:PuttingToUse rdf:about="http://iirds.tekom.de/iirds#GenericPuttingToUse">
		<rdfs:label xml:lang="de">In Nutzung nehmen</rdfs:label>
		<rdfs:label xml:lang="en">putting to use</rdfs:label>
		<iirds:description xml:lang="en">The PuttingToUse class is a parent class for the product lifecycle phases related to putting a product or technical system to use.</iirds:description>
		<rdfs:comment xml:lang="en">product life cycle phase after production in which a product is set up for its intended use</rdfs:comment>
	</iirds:PuttingToUse>
	<iirds:Reference rdf:about="http://iirds.tekom.de/iirds#GenericReference">
		<rdfs:label xml:lang="de">Referenz</rdfs:label>
		<rdfs:label xml:lang="en">reference</rdfs:label>
		<iirds:description xml:lang="en">The Reference class describes a topic type containing information that supports users as they perform a task, meaning data that is looked up rather than memorized. Examples are parameter lists, tables with technical data, UI control overviews, and parts lists. </iirds:description>
		<rdfs:comment xml:lang="en">topic type that provides additional details for lookup</rdfs:comment>
	</iirds:Reference>
	<iirds:Role rdf:about="http://iirds.tekom.de/iirds#GenericRole">
		<rdfs:label xml:lang="de">Rolle</rdfs:label>
		<rdfs:label xml:lang="en">role</rdfs:label>
		<iirds:description xml:lang="en">The Role class describes roles for users of the technical system and the associated technical information.</iirds:description>
		<rdfs:comment xml:lang="en">set of connected behaviors, privileges and obligations associated with a party</rdfs:comment>
	</iirds:Role>
	<iirds:Safety rdf:about="http://iirds.tekom.de/iirds#GenericSafety">
		<rdfs:label xml:lang="de">Sicherheit</rdfs:label>
		<rdfs:label xml:lang="en">safety</rdfs:label>
		<iirds:description xml:lang="en">The Safety class contains information subjects related to safety.</iirds:description>
		<rdfs:comment xml:lang="en">information subject that covers content which helps to avoid risk</rdfs:comment>
	</iirds:Safety>
	<iirds:SkillLevel rdf:about="http://iirds.tekom.de/iirds#GenericSkillLevel">
		<rdfs:label xml:lang="de">Kenntnisstufe</rdfs:label>
		<rdfs:label xml:lang="en">skill level</rdfs:label>
		<iirds:description xml:lang="en">The SkillLevel class describes custom skill levels that the users of the technical system and the associated technical information require.</iirds:description>
		<rdfs:comment xml:lang="en">degree of qualification of an individual</rdfs:comment>
	</iirds:SkillLevel>
	<iirds:Supply rdf:about="http://iirds.tekom.de/iirds#GenericSupply">
		<rdfs:label xml:lang="de">Hilfsmittel</rdfs:label>
		<rdfs:label xml:lang="en">generic supply</rdfs:label>
		<iirds:description xml:lang="en">The Supply class is a parent class for supplies that are required for working tasks described in technical documentation.</iirds:description>
		<rdfs:comment xml:lang="en">physical object used by an actor performing work tasks described in technical documentation</rdfs:comment>
	</iirds:Supply>
	<iirds:Task rdf:about="http://iirds.tekom.de/iirds#GenericTask">
		<rdfs:label xml:lang="de">Aufgabe</rdfs:label>
		<rdfs:label xml:lang="en">task</rdfs:label>
		<iirds:description xml:lang="en">Tasks provide instructions and may contain information on other aspects, such as requirements that must be fulfilled or safety instructions.</iirds:description>
		<rdfs:comment xml:lang="en">topic type that provides procedures and action steps to be followed or considered</rdfs:comment>
	</iirds:Task>
	<iirds:TechnicalData rdf:about="http://iirds.tekom.de/iirds#GenericTechnicalData">
		<rdfs:label xml:lang="de">Technische Daten</rdfs:label>
		<rdfs:label xml:lang="en">technical data</rdfs:label>
		<iirds:description xml:lang="en">Information that describes the technical characteristics of a product or component.</iirds:description>
		<rdfs:comment xml:lang="en">information subject that covers qualitative and quantitative characteristics  of technical objects</rdfs:comment>
	</iirds:TechnicalData>
	<iirds:TechnicalOverview rdf:about="http://iirds.tekom.de/iirds#GenericTechnicalOverview">
		<rdfs:label xml:lang="de">Technische Übersicht</rdfs:label>
		<rdfs:label xml:lang="en">technical overview</rdfs:label>
		<iirds:description xml:lang="en">The TechnicalOverview class is a parent class for information subjects describing contents related to technical plans, diagrams, or the technical architecture of the product.</iirds:description>
		<rdfs:comment xml:lang="en">information subject that covers the technical structure of a product</rdfs:comment>
	</iirds:TechnicalOverview>
	<iirds:Troubleshooting rdf:about="http://iirds.tekom.de/iirds#GenericTroubleshooting">
		<rdfs:label xml:lang="de">Störungsbeseitigung</rdfs:label>
		<rdfs:label xml:lang="en">troubleshooting</rdfs:label>
		<iirds:description xml:lang="en">Troubleshooting information may comprise a description of the symptoms, the cause of the error, and a remedy for the error.</iirds:description>
		<rdfs:comment xml:lang="en">topic type that provides an explanation on symptoms, diagnosis, and resolution of problems</rdfs:comment>
	</iirds:Troubleshooting>
	<iirds:Use rdf:about="http://iirds.tekom.de/iirds#GenericUse">
		<rdfs:label xml:lang="de">Nutzung</rdfs:label>
		<rdfs:label xml:lang="en">use</rdfs:label>
		<iirds:description xml:lang="en">The Use class is a parent class for product lifecycle phases related to using a product or technical system.</iirds:description>
		<rdfs:comment xml:lang="en">product life cycle phase in which the product is supposed to realize its function</rdfs:comment>
	</iirds:Use>
	<iirds:WorkingTime rdf:about="http://iirds.tekom.de/iirds#GenericWorkingTime">
		<rdfs:label xml:lang="de">Arbeitszeit</rdfs:label>
		<rdfs:label xml:lang="en">generic working time</rdfs:label>
		<iirds:description xml:lang="en">The WorkingTime class is a parent class for periods of time required for a specific working task.</iirds:description>
		<rdfs:comment xml:lang="en">period of time that is required for conducting a specific task</rdfs:comment>
		<iirds:duration rdf:datatype="http://www.w3.org/2001/XMLSchema#duration">PT0M</iirds:duration>
	</iirds:WorkingTime>
	<iirds:DirectoryNodeType rdf:about="http://iirds.tekom.de/iirds#Index">
		<rdfs:label xml:lang="de">Index</rdfs:label>
		<rdfs:label xml:lang="en">index</rdfs:label>
		<iirds:description xml:lang="en"/>
		<rdfs:comment xml:lang="en">directory node type that refers to an  ordered arrangement of entries, designed to enable users to locate information in information units</rdfs:comment>
	</iirds:DirectoryNodeType>
	<iirds:PuttingToUse rdf:about="http://iirds.tekom.de/iirds#Installation">
		<rdfs:label xml:lang="de">Installation</rdfs:label>
		<rdfs:label xml:lang="en">installation</rdfs:label>
		<iirds:description xml:lang="en"/>
		<rdfs:comment xml:lang="en">product life cycle phase of setting up a product in the designated target environment so that it fulfils its intended use</rdfs:comment>
	</iirds:PuttingToUse>
	<iirds:DocumentType rdf:about="http://iirds.tekom.de/iirds#InstallationInstructions">
		<rdfs:label xml:lang="de">Installationsanleitung</rdfs:label>
		<rdfs:label xml:lang="en">installation instructions</rdfs:label>
		<iirds:description xml:lang="en">For physical products: instructions enabling the operator to assemble and electrically connect a physical product so that it fulfills its intended use and does not endanger the health and safety of persons. For IT products: Instructions enabling the administrator to set up and potentially configure a program or new version on a computer so that does not endanger data security. </iirds:description>
		<rdfs:comment xml:lang="en">document type that refers to information on how to set up a product in the designated target environment so that it fulfils its intended use</rdfs:comment>
	</iirds:DocumentType>
	<iirds:Safety rdf:about="http://iirds.tekom.de/iirds#IntendedUse">
		<rdfs:label xml:lang="de">Bestimmungsgemäße Verwendung</rdfs:label>
		<rdfs:label xml:lang="en">intended use</rdfs:label>
		<iirds:description xml:lang="en"/>
		<rdfs:comment xml:lang="en">information subject that covers information which states the range of functions or foreseen applications defined and designed by the supplier of the product</rdfs:comment>
	</iirds:Safety>
	<iirds:Formality rdf:about="http://iirds.tekom.de/iirds#LegalInformation">
		<rdfs:label xml:lang="de">Rechtlicher Hinweis</rdfs:label>
		<rdfs:label xml:lang="en">legal information</rdfs:label>
		<iirds:description xml:lang="en"/>
		<rdfs:comment xml:lang="en">information subject that covers supplementary information referencing laws or regulations</rdfs:comment>
	</iirds:Formality>
	<iirds:Formality rdf:about="http://iirds.tekom.de/iirds#LicenceTerm">
		<rdfs:label xml:lang="de">Lizenzbedingung</rdfs:label>
		<rdfs:label xml:lang="en">license terms</rdfs:label>
		<iirds:description xml:lang="en"/>
		<rdfs:comment xml:lang="en">information subject that covers a legal contract between two parties wherein the property owner gives permission to another party to use its intellectual properties</rdfs:comment>
	</iirds:Formality>
	<iirds:DirectoryNodeType rdf:about="http://iirds.tekom.de/iirds#ListOfFigures">
		<rdfs:label xml:lang="de">Abbildungsverzeichnis</rdfs:label>
		<rdfs:label xml:lang="en">list of figures</rdfs:label>
		<iirds:synonym>LOF</iirds:synonym>
		<iirds:description xml:lang="en">Type of directory</iirds:description>
		<rdfs:comment xml:lang="en">directory node type that refers to a list of visuals and their location within information units, generally in order of appearance</rdfs:comment>
	</iirds:DirectoryNodeType>
	<iirds:DirectoryNodeType rdf:about="http://iirds.tekom.de/iirds#ListOfListings">
		<rdfs:label xml:lang="de">Codeverzeichnis</rdfs:label>
		<rdfs:label xml:lang="en">list of listings</rdfs:label>
		<iirds:synonym>LOL</iirds:synonym>
		<iirds:description xml:lang="en">Type of directory</iirds:description>
		<rdfs:comment xml:lang="en">directory node type that refers to a list of code snippets and their location within information units, generally in order of appearance</rdfs:comment>
	</iirds:DirectoryNodeType>
	<iirds:DirectoryNodeType rdf:about="http://iirds.tekom.de/iirds#ListOfTables">
		<rdfs:label xml:lang="de">Tabellenverzeichnis</rdfs:label>
		<rdfs:label xml:lang="en">list of tables</rdfs:label>
		<iirds:synonym>LOT</iirds:synonym>
		<iirds:description xml:lang="en">Type of directory</iirds:description>
		<rdfs:comment xml:lang="en">directory node type that refers to a list of tables and their location within information units, generally in order of appearance</rdfs:comment>
	</iirds:DirectoryNodeType>
	<iirds:Use rdf:about="http://iirds.tekom.de/iirds#Maintenance">
		<rdfs:label xml:lang="de">Wartung</rdfs:label>
		<rdfs:label xml:lang="en">maintenance</rdfs:label>
		<iirds:description xml:lang="en"/>
		<rdfs:comment xml:lang="en">product life cycle phase of activities intended  to retain or restore a system in or to operational state</rdfs:comment>
	</iirds:Use>
	<iirds:DocumentType rdf:about="http://iirds.tekom.de/iirds#MaintenanceInstructions">
		<rdfs:label xml:lang="de">Wartungsanleitung</rdfs:label>
		<rdfs:label xml:lang="en">maintenance instructions</rdfs:label>
		<iirds:description xml:lang="en"/>
		<rdfs:comment xml:lang="en">document type that refers to information on procedures to be followed to ensure that a product remains in good working order</rdfs:comment>
	</iirds:DocumentType>
	<iirds:Formality rdf:about="http://iirds.tekom.de/iirds#ManufacturerInformation">
		<rdfs:label xml:lang="de">Herstellerinformation</rdfs:label>
		<rdfs:label xml:lang="en">manufacturer information</rdfs:label>
		<iirds:description xml:lang="en"/>
		<rdfs:comment xml:lang="en">information subject that covers information on the manufacturer of the product</rdfs:comment>
	</iirds:Formality>
	<iirds:TechnicalOverview rdf:about="http://iirds.tekom.de/iirds#OperatingElement">
		<rdfs:label xml:lang="de">Bedienelement</rdfs:label>
		<rdfs:label xml:lang="en">control element</rdfs:label>
		<iirds:description xml:lang="en"/>
		<rdfs:comment xml:lang="en">information subject that covers interaction elements in user interface </rdfs:comment>
	</iirds:TechnicalOverview>
	<iirds:DocumentType rdf:about="http://iirds.tekom.de/iirds#OperatingInstructions">
		<rdfs:label xml:lang="de">Betriebsanleitung</rdfs:label>
		<rdfs:label xml:lang="en">operating instructions</rdfs:label>
		<iirds:description xml:lang="en">The instructions in this document type enable the user to operate a device, machine, or software considering the reference use as well as the safety and health regulations for the product.</iirds:description>
		<iirds:description xml:lang="de">Anleitung, die den Anwender dazu befähigt, ein Gerät, eine Maschine oder eine Software so zu betreiben, dass das Gerät oder die Maschine die bestimmungsgemäße Verwendung erfüllt und die Sicherheit und Gesundheit von Personen nicht beeinträchtigt wird.</iirds:description>
		<rdfs:comment xml:lang="en">document type that refers to information on the correct use of the product</rdfs:comment>
	</iirds:DocumentType>
	<iirds:Use rdf:about="http://iirds.tekom.de/iirds#Operation">
		<rdfs:label xml:lang="de">Betrieb</rdfs:label>
		<rdfs:label xml:lang="en">operation</rdfs:label>
		<iirds:description xml:lang="en"/>
		<rdfs:comment xml:lang="en">product life cycle phase in which a system carries out its designated functions</rdfs:comment>
	</iirds:Use>
	<iirds:DocumentType rdf:about="http://iirds.tekom.de/iirds#PartsCatalog">
		<rdfs:label xml:lang="de">Teilekatalog</rdfs:label>
		<rdfs:label xml:lang="en">parts catalog</rdfs:label>
		<iirds:description xml:lang="en"/>
		<rdfs:comment xml:lang="en">document type that refers to a list-style arrangement of spare part information</rdfs:comment>
	</iirds:DocumentType>
	<iirds:Formality rdf:about="http://iirds.tekom.de/iirds#ProductIdentification">
		<rdfs:label xml:lang="de">Produktidentifikation</rdfs:label>
		<rdfs:label xml:lang="en">product identification</rdfs:label>
		<iirds:description xml:lang="en"/>
		<rdfs:comment xml:lang="en">information subject that covers information on identity and characteristics of products</rdfs:comment>
	</iirds:Formality>
	<iirds:DesignAndRealization rdf:about="http://iirds.tekom.de/iirds#Production">
		<rdfs:label xml:lang="de">Herstellung</rdfs:label>
		<rdfs:label xml:lang="en">production</rdfs:label>
		<iirds:description xml:lang="en"/>
		<rdfs:comment xml:lang="en">product life cycle phase of manufacturing products</rdfs:comment>
	</iirds:DesignAndRealization>
	<iirds:Formality rdf:about="http://iirds.tekom.de/iirds#ProductName">
		<rdfs:label xml:lang="de">Produktbezeichnung</rdfs:label>
		<rdfs:label xml:lang="en">product name</rdfs:label>
		<iirds:description xml:lang="en"/>
		<rdfs:comment xml:lang="en">information subject that covers the designation of a product</rdfs:comment>
	</iirds:Formality>
	<iirds:DocumentType rdf:about="http://iirds.tekom.de/iirds#QuickGuide">
		<rdfs:label xml:lang="de">Kurzanleitung</rdfs:label>
		<rdfs:label xml:lang="en">quick reference guide</rdfs:label>
		<iirds:description xml:lang="en"/>
		<rdfs:comment xml:lang="en">document type that refers to selected information facilitating product use within a short period of time</rdfs:comment>
	</iirds:DocumentType>
	<iirds:Use rdf:about="http://iirds.tekom.de/iirds#Repair">
		<rdfs:label xml:lang="de">Reparatur</rdfs:label>
		<rdfs:label xml:lang="en">repair</rdfs:label>
		<iirds:description xml:lang="en"/>
		<rdfs:comment xml:lang="en">product life cycle phase of rectification of damages and malfunctions</rdfs:comment>
	</iirds:Use>
	<iirds:DocumentType rdf:about="http://iirds.tekom.de/iirds#RepairInstructions">
		<rdfs:label xml:lang="de">Reparaturanleitung</rdfs:label>
		<rdfs:label xml:lang="en">repair instructions</rdfs:label>
		<iirds:description xml:lang="en">The instructions in this document type enable the user to repair a device, machine, or system considering the reference use as well as the safety and health regulations for the product.</iirds:description>
		<iirds:description xml:lang="de">Anleitung, die den Anwender dazu befähigt, ein Gerät oder eine Maschine so instandzusetzen, dass das Gerät oder die Maschine die bestimmungsgemäße Verwendung erfüllt und die Sicherheit und Gesundheit von Personen nicht beeinträchtigt wird.</iirds:description>
		<rdfs:comment xml:lang="en">document type that refers to information on how to fix a failure of a product </rdfs:comment>
	</iirds:DocumentType>
	<iirds:DesignAndRealization rdf:about="http://iirds.tekom.de/iirds#RequirementsAnalysis">
		<rdfs:label xml:lang="de">Anforderungsanalyse</rdfs:label>
		<rdfs:label xml:lang="en">requirement analysis</rdfs:label>
		<iirds:description xml:lang="en"/>
		<rdfs:comment xml:lang="en">product life cycle phase in which understanding and prioritisation of necessary product characteristics is achieved</rdfs:comment>
	</iirds:DesignAndRealization>
	<iirds:Safety rdf:about="http://iirds.tekom.de/iirds#RestrictionOnUse">
		<rdfs:label xml:lang="de">Einsatzbeschränkungen</rdfs:label>
		<rdfs:label xml:lang="en">restriction on use</rdfs:label>
		<iirds:description xml:lang="en"/>
		<rdfs:comment xml:lang="en">information subject that covers information specifying under which conditions or in which manner the product shall not be used</rdfs:comment>
	</iirds:Safety>
	<iirds:Conformity rdf:about="http://iirds.tekom.de/iirds#RiskAssessment">
		<rdfs:label xml:lang="de">Risikobewertung</rdfs:label>
		<rdfs:label xml:lang="en">risk assessment</rdfs:label>
		<iirds:description xml:lang="en">A risk assessment determines the risks and hazards to life, environment, or machine functioning including a quantitative and qualitative estimate.</iirds:description>
		<rdfs:comment xml:lang="en">information subject covering a process comprising a risk analysis and risk evaluation of the product or their result</rdfs:comment>
	</iirds:Conformity>
	<iirds:Safety rdf:about="http://iirds.tekom.de/iirds#SafetyInstruction">
		<rdfs:label xml:lang="de">Sicherheitshinweis</rdfs:label>
		<rdfs:label xml:lang="en">safety instruction</rdfs:label>
		<iirds:description xml:lang="en"/>
		<rdfs:comment xml:lang="en">information subject covering general safety-related information applying to a range of information units</rdfs:comment>
	</iirds:Safety>
	<iirds:DocumentType rdf:about="http://iirds.tekom.de/iirds#SalesCatalog">
		<rdfs:label xml:lang="de">Verkaufskatalog</rdfs:label>
		<rdfs:label xml:lang="en">sales catalog</rdfs:label>
		<iirds:description xml:lang="en"/>
		<rdfs:comment xml:lang="en">document type that refers to a list-style arrangement of information relevant for product selection and ordering</rdfs:comment>
	</iirds:DocumentType>
	<iirds:Formality rdf:about="http://iirds.tekom.de/iirds#ScopeOfDelivery">
		<rdfs:label xml:lang="de">Lieferumfang</rdfs:label>
		<rdfs:label xml:lang="en">scope of delivery</rdfs:label>
		<iirds:description xml:lang="en"/>
		<rdfs:comment xml:lang="en">information subject that covers all work, services, materials, completed products, and documentation that the supplier shall provide to the purchaser according to the purchase order</rdfs:comment>
	</iirds:Formality>
	<iirds:Formality rdf:about="http://iirds.tekom.de/iirds#WarrantyConditions">
		<rdfs:label xml:lang="de">Garantiebedingungen</rdfs:label>
		<rdfs:label xml:lang="en">warranty conditions</rdfs:label>
		<iirds:description xml:lang="en"/>
		<rdfs:comment xml:lang="en">information subject that covers the specific terms of a promise given by a manufacturer or supplier to a purchaser to properly repair, replace or refund a faulty product</rdfs:comment>
	</iirds:Formality>
	<iirds:DocumentType rdf:about="http://iirds.tekom.de/iirds#Specification">
		<rdfs:label xml:lang="de">Spezifikation</rdfs:label>
		<rdfs:label xml:lang="en">specification</rdfs:label>
		<iirds:description xml:lang="en"/>
		<rdfs:comment xml:lang="en">document type that refers to information on technical properties of products</rdfs:comment>
	</iirds:DocumentType>
	<iirds:TechnicalOverview rdf:about="http://iirds.tekom.de/iirds#Symbol">
		<rdfs:label xml:lang="de">Symbol</rdfs:label>
		<rdfs:label xml:lang="en">symbol</rdfs:label>
		<iirds:description xml:lang="en"/>
		<rdfs:comment xml:lang="en">information subject that covers an assembly of visual designations, together with their names or explanations of their meaning</rdfs:comment>
	</iirds:TechnicalOverview>
	<iirds:DirectoryNodeType rdf:about="http://iirds.tekom.de/iirds#TableOfContents">
		<rdfs:label xml:lang="de">Inhaltsverzeichnis</rdfs:label>
		<rdfs:label xml:lang="en">table of contents</rdfs:label>
		<iirds:synonym>TOC</iirds:synonym>
		<iirds:description xml:lang="en">Directory type</iirds:description>
		<rdfs:comment xml:lang="en">directory node type that refers to a list of information units in logical order</rdfs:comment>
	</iirds:DirectoryNodeType>
	<iirds:Conformity rdf:about="http://iirds.tekom.de/iirds#TechnicalReport">
		<rdfs:label xml:lang="de">Technischer Bericht</rdfs:label>
		<rdfs:label xml:lang="en">technical report</rdfs:label>
		<iirds:description xml:lang="en"/>
		<rdfs:comment xml:lang="en">information subject covering a report of product conformity with legislative or normative requirements</rdfs:comment>
	</iirds:Conformity>
	<iirds:DocumentType rdf:about="http://iirds.tekom.de/iirds#TransportInstructions">
		<rdfs:label xml:lang="de">Transportanleitung</rdfs:label>
		<rdfs:label xml:lang="en">transport instructions</rdfs:label>
		<iirds:description xml:lang="en"/>
		<rdfs:comment xml:lang="en">document type that refers to instructions for the movement of products or their components from one location to another</rdfs:comment>
	</iirds:DocumentType>
	<iirds:DocumentType rdf:about="http://iirds.tekom.de/iirds#ElectronicIdentificationPlate">
		<rdfs:label xml:lang="de">Elektronisches Typenschild</rdfs:label>
		<rdfs:label xml:lang="en">electronic identification plate</rdfs:label>
		<iirds:description xml:lang="en">Type of document (VDI 2770)</iirds:description>
		<rdfs:comment xml:lang="en">document type referring electronically readable label on a product or component that provides information on its identity and characteristics</rdfs:comment>
	</iirds:DocumentType>
	<iirds:DocumentType rdf:about="http://iirds.tekom.de/iirds#Plan">
		<rdfs:label xml:lang="de">Plan</rdfs:label>
		<rdfs:label xml:lang="en">plan</rdfs:label>
		<iirds:description xml:lang="en">Type of document (VDI 2770).</iirds:description>
		<rdfs:comment xml:lang="en">document type that refers to technical plans for a component or machine</rdfs:comment>
	</iirds:DocumentType>
	<iirds:DocumentType rdf:about="http://iirds.tekom.de/iirds#Certificate">
		<rdfs:label xml:lang="de">Zertifikat</rdfs:label>
		<rdfs:label xml:lang="en">certificate</rdfs:label>
		<iirds:description xml:lang="en">Type of document (VDI 2770). Examples are ATEX certificates, acceptance reports, and material certificates.</iirds:description>
		<rdfs:comment xml:lang="en">document type that refers to a document attesting conformity with applicable regulations</rdfs:comment>
	</iirds:DocumentType>
	<iirds:DocumentType rdf:about="http://iirds.tekom.de/iirds#SafetyInstructions">
		<rdfs:label xml:lang="de">Sicherheitsanleitung</rdfs:label>
		<rdfs:label xml:lang="en">safety instructions</rdfs:label>
		<iirds:description xml:lang="en">Type of document (VDI 2770). Examples are documents about the intended use of the product, protection/safety measures, safety equipment, and explosion prevention. </iirds:description>
		<rdfs:comment xml:lang="en">document type that refers to safety-related information</rdfs:comment>
	</iirds:DocumentType>
	<iirds:DocumentType rdf:about="http://iirds.tekom.de/iirds#BillOfMaterials">
		<rdfs:label xml:lang="de">Stückliste</rdfs:label>
		<rdfs:label xml:lang="en">bill of materials</rdfs:label>
		<iirds:description xml:lang="en">Type of document (VDI 2770). Examples are part list with part number, part description, order number, and references to other documents.</iirds:description>
		<rdfs:comment xml:lang="en">document type that refers to formal tabulation of the physical assemblies, subassemblies, and components needed to fabricate a product</rdfs:comment>
	</iirds:DocumentType>
	<iirds:DocumentType rdf:about="http://iirds.tekom.de/iirds#ContractualDocument">
		<rdfs:label xml:lang="de">Vertragliches Dokument</rdfs:label>
		<rdfs:label xml:lang="en">contractual document</rdfs:label>
		<iirds:description xml:lang="en">Type of document (VDI 2770). Contractual documents include, among others, contracts, acceptance reports, and service conditions.</iirds:description>
		<rdfs:comment xml:lang="en">document type that refers to a binding agreement between parties</rdfs:comment>
	</iirds:DocumentType>
	<iirds:DocumentType rdf:about="http://iirds.tekom.de/iirds#TechnicalDrawingDiagram">
		<rdfs:label xml:lang="de">Technische Zeichnung/Diagramm</rdfs:label>
		<rdfs:label xml:lang="en">technical drawing/diagram</rdfs:label>
		<rdfs:comment xml:lang="en">document type that refers to a visual that conveys information about how an object functions or is constructed</rdfs:comment>
		<iirds:description xml:lang="en">A technical drawing or diagram.</iirds:description>
	</iirds:DocumentType>
	<iirds:DocumentType rdf:about="http://iirds.tekom.de/iirds#IdentificationDocument">
		<rdfs:label xml:lang="de">Identifikationsdokument</rdfs:label>
		<rdfs:label xml:lang="en">identification document</rdfs:label>
		<rdfs:comment xml:lang="en">document type that refers to information on identity and characteristics of products</rdfs:comment>
		<iirds:description xml:lang="en">Identifies an object and provides descriptive or classifying information.</iirds:description>
	</iirds:DocumentType>
	<iirds:WarningMessage rdf:about="http://iirds.tekom.de/iirds#Danger">
		<rdfs:label xml:lang="de">Gefahr</rdfs:label>
		<rdfs:label xml:lang="en">danger</rdfs:label>
		<iirds:description xml:lang="en">See ANSI Z535.5</iirds:description>
		<rdfs:comment xml:lang="en">warning message that describes a hazardous situation which, if not avoided, will result in death or serious injury</rdfs:comment>
	</iirds:WarningMessage>
	<iirds:WarningMessage rdf:about="http://iirds.tekom.de/iirds#Warning">
		<rdfs:label xml:lang="de">Warnung</rdfs:label>
		<rdfs:label xml:lang="en">warning</rdfs:label>
		<iirds:description xml:lang="en">See ANSI Z535.5</iirds:description>
		<rdfs:comment xml:lang="en">warning message that describes a hazardous situation which, if not avoided, could result in death or serious injury</rdfs:comment>
	</iirds:WarningMessage>
	<iirds:WarningMessage rdf:about="http://iirds.tekom.de/iirds#Caution">
		<rdfs:label xml:lang="de">Vorsicht</rdfs:label>
		<rdfs:label xml:lang="en">caution</rdfs:label>
		<iirds:description xml:lang="en">See ANSI Z535.5</iirds:description>
		<rdfs:comment xml:lang="en">warning message that describes a hazardous situation which, if not avoided, could result in minor or moderate injury</rdfs:comment>
	</iirds:WarningMessage>
	<iirds:WarningMessage rdf:about="http://iirds.tekom.de/iirds#Notice">
		<rdfs:label xml:lang="de">Hinweis</rdfs:label>
		<rdfs:label xml:lang="en">notice</rdfs:label>
		<iirds:description xml:lang="en">See ANSI Z535.5</iirds:description>
		<rdfs:comment xml:lang="en">message that contains information considered important but not related to personal injury</rdfs:comment>
	</iirds:WarningMessage>
	<iirds:WarningMessage rdf:about="http://iirds.tekom.de/iirds#GenericWarningMessage">
		<rdfs:label xml:lang="de">Warnhinweis</rdfs:label>
		<rdfs:label xml:lang="en">warning message</rdfs:label>
		<iirds:description xml:lang="en">If possible, use Danger, Warning, Caution, or Notice instead.</iirds:description>
		<rdfs:comment xml:lang="en">safety-related information that warns about hazards and instructs on how to avoid them</rdfs:comment>
	</iirds:WarningMessage>
	<iirds:IdentityType rdf:about="http://iirds.tekom.de/iirds#ArticleCode">
		<rdfs:label xml:lang="de">Artikelcode</rdfs:label>
		<rdfs:label xml:lang="en">article code</rdfs:label>
		<iirds:description xml:lang="en">Examples of article code are material number, article number, or item number.</iirds:description>
		<rdfs:comment xml:lang="en">identity type of the manufacturer's reference number or other identifier for products or for parts of a product</rdfs:comment>
	</iirds:IdentityType>
	<iirds:IdentityType rdf:about="http://iirds.tekom.de/iirds#OrderCode">
		<rdfs:label xml:lang="de">Bestellcode</rdfs:label>
		<rdfs:label xml:lang="en">order code</rdfs:label>
		<iirds:description xml:lang="en">Examples of order code are configuration number, product number, or code.</iirds:description>
		<rdfs:comment xml:lang="en">identity type of the manufacturer's unique procurement key</rdfs:comment>
	</iirds:IdentityType>
	<iirds:IdentityType rdf:about="http://iirds.tekom.de/iirds#ProductType">
		<rdfs:label xml:lang="de">Produkttyp</rdfs:label>
		<rdfs:label xml:lang="en">product type</rdfs:label>
		<iirds:description xml:lang="en">Examples of product type are labels of product variants and type or model.</iirds:description>
		<rdfs:comment xml:lang="en">identity type for products of the same series</rdfs:comment>
	</iirds:IdentityType>
	<iirds:IdentityType rdf:about="http://iirds.tekom.de/iirds#GlobalTradeItemNumber">
		<rdfs:label xml:lang="de">GTIN</rdfs:label>
		<rdfs:label xml:lang="en">GTIN</rdfs:label>
		<iirds:description xml:lang="en">Global Trade Item Number (GTIN) is an identifier for trade items.</iirds:description>
		<rdfs:comment xml:lang="en">identity type of internationally coordinated, uniform and globally unique article number for products and services</rdfs:comment>
	</iirds:IdentityType>
	<iirds:IdentityType rdf:about="http://iirds.tekom.de/iirds#EuropeanArticleNumber">
		<rdfs:label xml:lang="de">EAN</rdfs:label>
		<rdfs:label xml:lang="en">EAN</rdfs:label>
		<iirds:description xml:lang="en">European Article Number (EAN; also International Article Number, IAN) identifier for trade items.</iirds:description>
		<rdfs:comment xml:lang="en">identity type of the European article number according to ISO/IEC 15420</rdfs:comment>
	</iirds:IdentityType>
	<iirds:IdentityType rdf:about="http://iirds.tekom.de/iirds#ObjectInstanceURI">
		<rdfs:label xml:lang="de">Instanz einer Objekt-URI</rdfs:label>
		<rdfs:label xml:lang="en">instance of object URI</rdfs:label>
		<iirds:description xml:lang="en">A globally biunique serial number, for example, according to the stipulations made in DIN SPEC 91406.</iirds:description>
		<rdfs:comment xml:lang="en">identity type of the globally unique URI for the product instance</rdfs:comment>
	</iirds:IdentityType>
	<iirds:IdentityType rdf:about="http://iirds.tekom.de/iirds#SerialNumber">
		<rdfs:label xml:lang="de">Seriennummer</rdfs:label>
		<rdfs:label xml:lang="en">serial number</rdfs:label>
		<iirds:description xml:lang="en">A serial number, serial ID oder serial code identifying a single object instance.</iirds:description>
		<rdfs:comment xml:lang="en">identity type of the number used to identify an individual product instance</rdfs:comment>
	</iirds:IdentityType>
	<iirds:ClassificationType rdf:about="http://iirds.tekom.de/iirds#EclassCodedName">
		<rdfs:label xml:lang="de">ECLASS Coded Name</rdfs:label>
		<rdfs:label xml:lang="en">ECLASS Coded Name</rdfs:label>
		<iirds:description xml:lang="en">classification type that references an ECLASS product classification by an international registration data identifier (IRDI) path</iirds:description>
		<rdfs:comment xml:lang="en">8-digit class code that references an ECLASS product classification</rdfs:comment>
	</iirds:ClassificationType>
	<iirds:ClassificationType rdf:about="http://iirds.tekom.de/iirds#EclassIRDI">
		<rdfs:label xml:lang="de">ECLASS IRDI</rdfs:label>
		<rdfs:label xml:lang="en">ECLASS IRDI</rdfs:label>
		<rdfs:comment xml:lang="en">classification type that references an ECLASS product classification by an international registration data identifier (IRDI) path</rdfs:comment>
	</iirds:ClassificationType>
	<iirds:ClassificationType rdf:about="http://iirds.tekom.de/iirds#CDD">
		<rdfs:label xml:lang="de">CDD Identifikator</rdfs:label>
		<rdfs:label xml:lang="en">CDD identifier</rdfs:label>
		<rdfs:comment xml:lang="en">classification type that references a product classification in the Common Data Dictionary (CDD, IEC 61360)</rdfs:comment>
	</iirds:ClassificationType>
</rdf:RDF>
